Merge with James' hounours work 2/x: fix projection/proofs
Co-authored-by: James Shaker <james.shaker@gmail.com>

projection/proofs/to_cake/lib_tools/state_tacticLib.sml
@@ -1,0 +1,101 @@
+structure state_tacticLib :> state_tacticLib =
+	struct
+	open HolKernel Tactical;
+	(* Reduce right-assoc addition term to list of all free
+	   variables in sequence until non-variable or bound variable
+	   found *)
+	fun get_add_terms (bvs,t) =
+		case Lib.total numSyntax.dest_plus t of
+			NONE       => []
+		|   SOME (l,r) =>
+				if Term.is_var l andalso not (boolLib.tmem l bvs) then
+					l::get_add_terms (bvs,r)
+				else
+					[]
+
+	(* Fail if any given variable is free in assumptions or goal *)
+	fun fail_if_free vars (G as (asl,w)) =
+		let
+			val all_free = flatten ((Term.free_vars w)::(map Term.free_vars asl))
+		in
+			(if null(Lib.op_intersect Term.aconv vars all_free) then
+				ALL_TAC
+			else
+				NO_TAC) G
+		end 
+
+	(* Take an abbreviated left-assoc addition and return a theorem tactic
+	   to rewrite the right-assoc version of the abbreviated addition *)
+	fun genpmc th =
+	let
+		val mc          = Term.genvar “:num”
+	in
+		Rewrite.REWRITE_RULE [markerTheory.Abbrev_def] th |> Thm.SYM |>
+							  Thm.AP_TERM numSyntax.plus_tm |> Lib.C Thm.AP_THM mc
+							  |> Rewrite.REWRITE_RULE [Conv.GSYM arithmeticTheory.ADD_ASSOC]
+							  |> Thm.GEN mc |> (fn th => Rewrite.PURE_REWRITE_TAC[th])
+	end
+
+
+	fun unite_nums nm (G as (asl,w)) =
+	let
+		(* tripaddP behaviour:
+			- Try and match given term to right-assoc addition
+				1. If NONE then return NONE
+				2. If SOME match then:
+					a. Retrieve x, y, and z variables
+					b. Check x and y are free variables
+						-> If False then return NONE
+					c. Run get_add_terms to retrieve all added
+					   free variables in z
+					d. Create left-assoc addition of free variable
+					   sequence
+					e. Return SOME tactic to abbreviate left-assoc addition of found
+					   free variables and the list of variables used in abbreviation *)
+		val x = Term.genvar “:num”
+		val y = Term.genvar “:num”
+		val z = Term.genvar “:num”
+		fun tripaddP (bvs,t) =
+			case Lib.total (Term.match_term ``^x + (^y + ^z)``) t of
+				SOME (theta,_) =>
+				let
+					val x_v   = valOf (Lib.subst_assoc (Term.aconv x) theta)
+					val y_v   = valOf (Lib.subst_assoc (Term.aconv y) theta)
+					val xy_vs = [x_v,y_v]
+					val z_v   = valOf (Lib.subst_assoc (Term.aconv z) theta)
+				in
+					if (List.all Term.is_var xy_vs) andalso
+					   null(Lib.op_intersect Term.aconv bvs xy_vs) then
+					   let
+					   	val z_vars   = get_add_terms (bvs,z_v)
+					   	val xyz_vars = x_v::y_v::z_vars
+					   	val arhs     = numSyntax.list_mk_plus xyz_vars
+					   	val atac     = Q.ABBREV_TAC [QUOTE ("UNITE_NUMS_TEMP = "),ANTIQUOTE arhs]
+					   in
+					   	SOME (atac,xyz_vars)
+					   end
+					else
+						NONE
+				end
+			|	NONE 		   => NONE
+	in
+		(* Behaviour:
+		   - Try and find a subterm that tripaddP can produce tactic from.
+		 		1. If NONE then fail.
+		 		2. If SOME then:
+		 			a. Apply abbreviation tactic to combined added numbers
+		 			b. Use genpmc to handle right associated addition of
+		 			   same numbers
+		 			c. Check when addition of vars destroyed no free
+		 			   versions elsewhere of some remain
+		 			d. Rename UNITE_NUMS_TEMP to given nm with Abbrev
+		 			e. Remove remaining Abbrev to just leave behind the
+		 			   rename *)
+		case gen_find_term tripaddP w of
+			NONE    => NO_TAC
+		| 	SOME (atac,vars) => atac >> first_x_assum genpmc >> (fail_if_free vars) >>
+		                        Q.ABBREV_TAC [QUOTE (nm ^ " = "),QUOTE "UNITE_NUMS_TEMP"] >>
+		                        first_x_assum (K ALL_TAC)
+	end G
+
+	end;
