semantics/proofs/payloadPropsScript.sml
@@ -32,11 +32,29 @@ Theorem DRESTRICT_normalise_queues:
 Proof
   rw[normalise_queues_def,fmap_eq_flookup,FLOOKUP_DRESTRICT] >> rw[] >> fs[]
 QED
-        
+
 Theorem normalised_qpush[simp]:
   normalised q ⇒ normalised(qpush q p d)
 Proof
   rw[normalised_def]
+QED
+
+Theorem qlk_update[simp]:
+  qlk (q |+ (p,x)) p = x
+Proof
+  EVAL_TAC
+QED
+
+Theorem qlk_update2[simp]:
+  p1 ≠ p2 ⇒ qlk (q |+ (p1,x)) p2 = qlk q p2
+Proof
+  EVAL_TAC >> rw[]
+QED
+
+Theorem qlk_FEMPTY[simp]:
+  qlk FEMPTY p = []
+Proof
+  EVAL_TAC
 QED
 
 Theorem normalise_queues_FUPDATE_NONEMPTY:
@@ -81,7 +99,7 @@ Proof
   ho_match_mp_tac trans_ind >>
   rw[normalised_network_def]
 QED
-        
+
 (* todo: move? *)
 val EXISTS_REPLICATE = Q.store_thm("EXISTS_REPLICATE",
   `!f n d. EXISTS f (REPLICATE n d) = (n > 0 /\ f d)`,
@@ -142,7 +160,13 @@ val trans_enqueue' = Q.store_thm("trans_enqueue'",
 Theorem qlk_qpush[simp]:
   qlk (qpush q p1 d) p1 = qlk q p1 ++ [d]
 Proof
-  rw[qlk_def,qpush_def,fget_def,FLOOKUP_UPDATE]  
+  rw[qlk_def,qpush_def,fget_def,FLOOKUP_UPDATE]
+QED
+
+Theorem normalise_queues_FUPDATE_FUPDATE[simp]:
+  normalise_queues(q |+ (p,d)) |+ (p,d') = normalise_queues q |+ (p,d')
+Proof
+  rw[fmap_eq_flookup,normalise_queues_def,FLOOKUP_DRESTRICT,FLOOKUP_UPDATE]
 QED
 
 Theorem trans_dequeue_last_payload':
@@ -407,7 +431,7 @@ Proof
   pop_assum(qspec_then ‘p1’ mp_tac) >> rw[qlk_def,fget_def] >>
   FULL_CASE_TAC >> fs[]
 QED
-        
+
 Theorem trans_no_selfloop:
   !conf p1 alpha p2.
   trans conf p1 alpha p2 /\ conf.payload_size > 0
@@ -534,6 +558,1634 @@ Theorem intermediate_final_IMP:
   !d. intermediate d /\ final d ==> F
 Proof
   Cases >> rpt strip_tac >> fs[intermediate_def,final_def] >> rveq >> fs[]
+QED
+
+Theorem qpush_prefix:
+  ∀qs spL spA dA.
+    isPREFIX (qlk qs spL) (qlk (qpush qs spA dA) spL)
+Proof
+  rw[qlk_def,qpush_def,fget_def] >>
+  Cases_on ‘spL = spA’ >>
+  rw[finite_mapTheory.FLOOKUP_UPDATE] >>
+  Cases_on ‘FLOOKUP qs spA’ >> rw[rich_listTheory.IS_PREFIX_SNOC]
+QED
+
+(* Pushing to different sender queues is commutative *)
+Theorem qpush_commutes:
+  ∀qs spA dA spB dB.
+    spA ≠ spB ⇒
+      qpush (qpush qs spA dA) spB dB =
+      qpush (qpush qs spB dB) spA dA
+Proof
+  rw[qpush_def,qlk_def,fget_def,finite_mapTheory.FLOOKUP_UPDATE] >>
+  metis_tac[finite_mapTheory.FUPDATE_COMMUTES]
+QED
+
+(* Message can't be final and intermediate *)
+Theorem final_inter_mutexc:
+  ∀d. ¬(intermediate d ∧ final d)
+Proof
+  Cases_on ‘d’ >>
+  rw[intermediate_def,final_def] >>
+  Cases_on ‘h ≠ 2w’ >> fs[] >>
+  rw[wordsTheory.dimword_def,wordsTheory.dimindex_8]
+QED
+
+(* PAYLOAD NETWORK INVARIANTS *)
+(* Contained Nodes *)
+Definition net_has_node_def:
+  (net_has_node NNil              _  = F)                          ∧
+  (net_has_node (NPar n1 n2)      nd = (net_has_node n1 nd ∨
+                                        net_has_node n2 nd   )) ∧
+  (net_has_node (NEndpoint p _ _) nd = (p = nd))
+End
+
+Theorem trans_pres_nodes:
+  ∀conf s0 l s1.
+    trans conf s0 l s1 ⇒
+      (∀nd. net_has_node s0 nd ⇔ net_has_node s1 nd)
+Proof
+  Induct_on ‘trans’ >> rw[net_has_node_def]
+QED
+
+(* Wellformedness *)
+Definition net_wf_def:
+  (net_wf NNil = T) ∧
+  (net_wf (NEndpoint _ _ _) = T) ∧
+  (net_wf (NPar n1 n2) ⇔ net_wf n1 ∧ net_wf n2 ∧
+                         DISJOINT
+                          (net_has_node n1)
+                          (net_has_node n2))
+End
+
+Theorem trans_pres_wf:
+  ∀conf s0 l s1.
+    trans conf s0 l s1 ⇒
+      (net_wf s0 ⇔ net_wf s1)
+Proof
+  Induct_on ‘trans’ >>
+  rw[net_wf_def] >>
+  metis_tac[trans_pres_nodes,EQ_IMP_THM]
+QED
+
+(* PAYLOAD NETWORK COMMUNICATION PROPERTIES *)
+(* Necessary and Sufficient Network Receieve Conditions *)
+Theorem trans_receive_cond:
+  ∀conf sp N d dp.
+    (sp ≠ dp ∧ net_has_node N dp) ⇔
+    (∃N'. trans conf N (LReceive sp d dp) N')
+Proof
+  rw[EQ_IMP_THM]
+  >- (Induct_on ‘N’ >> rw[net_has_node_def] >> metis_tac[trans_rules])
+  >- (first_x_assum mp_tac >> Induct_on ‘trans’ >> rw[net_has_node_def])
+  >- (first_x_assum mp_tac >> Induct_on ‘trans’ >> rw[net_has_node_def])
+QED
+
+(* Necessary Network Sending Conditions *)
+Theorem trans_send_cond:
+  ∀conf sp N d dp.
+    (∃N'. trans conf N (LSend sp d dp) N') ⇒
+    (sp ≠ dp ∧ net_has_node N sp)
+Proof
+  rw[] >> first_x_assum mp_tac >>
+  Induct_on ‘trans’ >> rw[net_has_node_def]
+QED
+
+(* Well-formed Network Sending is unique *)
+Theorem trans_send_unique:
+  ∀conf N1 aN2 bN2 sp rp da db.
+    net_wf N1 ∧
+    trans conf N1 (LSend sp da rp) aN2 ∧
+    trans conf N1 (LSend sp db rp) bN2 ⇒
+    da = db
+Proof
+  Induct_on ‘N1’
+  >- (rw[] >>
+      ‘net_has_node NNil sp’
+        by metis_tac[trans_send_cond] >>
+      fs[net_has_node_def])
+  >- (rw[] >>
+      fs[net_wf_def] >>
+      rpt (qpat_x_assum ‘trans _ (NPar _ _) _ _’
+           (assume_tac o ONCE_REWRITE_RULE [trans_cases])) >>
+      fs[]
+      >- rpt (first_x_assum (dxrule_then strip_assume_tac))
+      >- (rename1 ‘DISJOINT (net_has_node N1A) (net_has_node N1B)’ >>
+          ‘sp ∈ net_has_node N1A ∧ sp ∈ net_has_node N1B’
+            suffices_by (rw[] >>
+                        fs[IN_DISJOINT] >>
+                        first_x_assum (qspec_then ‘sp’ assume_tac) >>
+                        rfs[]) >>
+          metis_tac[trans_send_cond,IN_APP])
+      >- (rename1 ‘DISJOINT (net_has_node N1A) (net_has_node N1B)’ >>
+          ‘sp ∈ net_has_node N1A ∧ sp ∈ net_has_node N1B’
+            suffices_by (rw[] >>
+                        fs[IN_DISJOINT] >>
+                        first_x_assum (qspec_then ‘sp’ assume_tac) >>
+                        rfs[]) >>
+          metis_tac[trans_send_cond,IN_APP])
+      >- rpt (first_x_assum (dxrule_then strip_assume_tac)))
+  >- (rw[] >>
+      ntac 2 (fs[Once trans_cases]) >>
+      rfs[])
+QED
+
+(* CONFLUENCE *)
+(* Restrictions of wf labels for confluence *)
+Definition wf_label_def:
+  wf_label N L =
+    case L of
+      LSend    sp d rp => ¬(net_has_node N rp)
+    | LReceive sp d rp => ¬(net_has_node N sp)
+    | LTau             => T
+End
+
+(* Restrictions of compatible labels for confluence *)
+Definition compat_labels_def:
+  compat_labels LA LB =
+    ∀sp1 d1 rp1 sp2 d2 rp2.
+      (LA = LReceive sp1 d1 rp1) ∧
+      (LB = LReceive sp2 d2 rp2) ⇒
+      (sp1 ≠ sp2 ∨ d1 = d2 ∨ rp1 ≠ rp2)
+End
+
+(* Basic theorem about generating compatible receive labels *)
+Theorem send_gen_compat:
+  ∀N1 N2A N2B spA dA rpA spB dB rpB.
+    net_wf N1 ∧
+    trans conf N1 (LSend spA dA rpA) N2A ∧
+    trans conf N1 (LSend spB dB rpB) N2B ⇒
+    compat_labels (LReceive spA dA rpA) (LReceive spB dB rpB)
+Proof
+  simp[compat_labels_def] >>
+  Induct_on ‘N1’
+  >- rw[Once trans_cases]
+  >- (rw[] >>
+      rename [‘net_wf (NPar N1a N1b)’] >>
+      ‘net_wf N1a ∧ net_wf N1b’
+        by fs[net_wf_def] >>
+      fs[] >>
+      rpt (qpat_x_assum ‘trans conf (NPar _ _) _ _’
+                        (assume_tac o ONCE_REWRITE_RULE [trans_cases])) >>
+      fs[] >> TRY (metis_tac []) >> CCONTR_TAC >>
+      ‘net_has_node N1a spA ∧ net_has_node N1b spA’
+        suffices_by metis_tac[net_wf_def,
+                              DISJOINT_SYM,
+                              DISJOINT_ALT,
+                              IN_APP] >>
+      metis_tac[trans_send_cond])
+  >- (rw[Once trans_cases] >>
+      fs[Once trans_cases] >>
+      fs[])
+QED
+
+(*  Confluence Result for different Labels *)
+Theorem trans_diff_diamond:
+  ∀N1 LA N2A LB N2B.
+    net_wf N1 ∧
+    wf_label N1 LA ∧
+    wf_label N1 LB ∧
+    LA ≠ LB ∧
+    compat_labels LA LB ∧
+    trans conf N1 LA N2A ∧
+    trans conf N1 LB N2B ⇒
+    ∃N3.
+      trans conf N2A LB N3 ∧
+      trans conf N2B LA N3
+Proof
+  Induct_on ‘trans’ >>
+  rw[] >> pop_assum (fn x => strip_assume_tac(REWRITE_RULE [Once trans_cases] x)) >>
+  fs[] >> rw[] >> fs[compat_labels_def]
+  (* LSend Final/LRecieve *)
+  >- (rename [‘NEndpoint c s e’,‘NEndpoint _ (_ with queues := _) _’,‘LReceive sp rd c’] >>
+      qmatch_goalsub_abbrev_tac ‘s with queues := nqs’ >>
+      qexists_tac ‘NEndpoint c (s with queues := nqs) e’ >>
+      rw[]
+      >- metis_tac[trans_rules]
+      >- (irule (hd (CONJUNCTS trans_rules)) >>
+          simp[]))
+  (* LSend Intermediate/LRecieve *)
+  >- (rename [‘Send rp sv n e’,‘Send rp sv (n + _) e’,
+             ‘LReceive sp rd c’] >>
+      qmatch_goalsub_abbrev_tac ‘s with queues := nqs’ >>
+      qexists_tac ‘NEndpoint c (s with queues := nqs) (Send rp sv (n + conf.payload_size) e)’ >>
+      rw[]
+      >- metis_tac[trans_rules]
+      >- (irule (el 2 (CONJUNCTS trans_rules)) >>
+         simp[]))
+  (* LRecieve/LSend Final *)
+  >- (rename [‘NEndpoint c s e’,‘NEndpoint _ (_ with queues := _) _’,‘LReceive sp rd c’] >>
+      qmatch_goalsub_abbrev_tac ‘s with queues := nqs’ >>
+      qexists_tac ‘NEndpoint c (s with queues := nqs) e’ >>
+      rw[]
+      >- (irule (hd (CONJUNCTS trans_rules)) >>
+          simp[])
+      >- metis_tac[trans_rules])
+  (* LRecieve/LSend Intermediate *)
+  >- (rename [‘Send rp sv n e’,‘Send rp sv (n + _) e’,
+             ‘LReceive sp rd c’] >>
+      qmatch_goalsub_abbrev_tac ‘s with queues := nqs’ >>
+      qexists_tac ‘NEndpoint c (s with queues := nqs) (Send rp sv (n + conf.payload_size) e)’ >>
+      rw[]
+      >- (irule (el 2 (CONJUNCTS trans_rules)) >>
+         simp[])
+      >- metis_tac[trans_rules])
+  (* LReceive/LReceive *)
+  >- (rename [‘LReceive sp1 d1 c’,‘sp1 = sp2 ⇒ d2 = d1’] >>
+      Cases_on ‘sp1 = sp2’
+      >- fs[]
+      >- (qexists_tac ‘NEndpoint c (s with queues := qpush (qpush s.queues sp1 d1) sp2 d2) e’ >>
+          rw[]
+          >- (qspecl_then [‘s.queues’,‘sp1’,‘d1’,‘sp2’,‘d2’] assume_tac
+                          qpush_commutes >>
+              rfs[] >> first_x_assum SUBST1_TAC >>
+              qmatch_goalsub_abbrev_tac ‘trans conf (NEndpoint c os e) _ _’ >>
+              ‘qpush s.queues sp2 d2 = os.queues’
+                by rw[Abbr ‘os’] >>
+              first_x_assum SUBST1_TAC >>
+              qmatch_goalsub_abbrev_tac ‘trans _ _ _ (NEndpoint _ ns _)’ >>
+              ‘ns = os with queues := qpush os.queues sp1 d1’
+                by rw[Abbr ‘ns’,Abbr ‘os’] >>
+              metis_tac[trans_rules])
+          >- (qmatch_goalsub_abbrev_tac ‘trans conf (NEndpoint c os e) _ _’ >>
+              ‘qpush s.queues sp1 d1 = os.queues’
+                by rw[Abbr ‘os’] >>
+              first_x_assum SUBST1_TAC >>
+              qmatch_goalsub_abbrev_tac ‘trans _ _ _ (NEndpoint _ ns _)’ >>
+              ‘ns = os with queues := qpush os.queues sp2 d2’
+                by rw[Abbr ‘ns’,Abbr ‘os’] >>
+              metis_tac[trans_rules])))
+  (* LReceive/LReceive *)
+  >- (rename [‘LReceive sp1 d1 c’,‘sp1 = sp2 ⇒ d2 = d1’] >>
+      Cases_on ‘sp1 = sp2’
+      >- fs[]
+      >- (qexists_tac ‘NEndpoint c (s with queues := qpush (qpush s.queues sp1 d1) sp2 d2) e’ >>
+          rw[]
+          >- (qspecl_then [‘s.queues’,‘sp1’,‘d1’,‘sp2’,‘d2’] assume_tac
+                          qpush_commutes >>
+              rfs[] >> first_x_assum SUBST1_TAC >>
+              qmatch_goalsub_abbrev_tac ‘trans conf (NEndpoint c os e) _ _’ >>
+              ‘qpush s.queues sp2 d2 = os.queues’
+                by rw[Abbr ‘os’] >>
+              first_x_assum SUBST1_TAC >>
+              qmatch_goalsub_abbrev_tac ‘trans _ _ _ (NEndpoint _ ns _)’ >>
+              ‘ns = os with queues := qpush os.queues sp1 d1’
+                by rw[Abbr ‘ns’,Abbr ‘os’] >>
+              metis_tac[trans_rules])
+          >- (qmatch_goalsub_abbrev_tac ‘trans conf (NEndpoint c os e) _ _’ >>
+              ‘qpush s.queues sp1 d1 = os.queues’
+                by rw[Abbr ‘os’] >>
+              first_x_assum SUBST1_TAC >>
+              qmatch_goalsub_abbrev_tac ‘trans _ _ _ (NEndpoint _ ns _)’ >>
+              ‘ns = os with queues := qpush os.queues sp2 d2’
+                by rw[Abbr ‘ns’,Abbr ‘os’] >>
+              metis_tac[trans_rules])))
+  (* LReceive/LTau (Receive Final) *)
+  >- (rename [‘NEndpoint c (s with queues := _) (Receive sp2 sv2 ds2 e)’,
+              ‘LReceive sp d c’] >>
+      qmatch_goalsub_abbrev_tac ‘<|bindings := fb; queues := bfq |>’ >>
+      qexists_tac ‘NEndpoint c <|bindings := fb; queues := qpush bfq sp d|> e’ >>
+      rw[]
+      >- (qunabbrev_tac ‘bfq’ >> qunabbrev_tac ‘fb’ >>
+          qmatch_goalsub_abbrev_tac ‘trans _ (NEndpoint _ sq (Receive _ _ _ _)) _
+                                             (NEndpoint _ ns _)’ >>
+          rename1 ‘qlk s.queues sp2 = dr::tl’ >>
+          ‘∃tln. qlk sq.queues sp2 = dr::tln’
+            by (qunabbrev_tac ‘sq’ >>
+                fs[qlk_def,fget_def,qpush_def,finite_mapTheory.FLOOKUP_UPDATE] >>
+                Cases_on ‘sp = sp2’ >> Cases_on ‘FLOOKUP s.queues sp2’ >>
+                fs[] >> metis_tac[]) >>
+          ‘ns = sq with
+                <|queues := normalise_queues(sq.queues |+ (sp2,tln));
+                  bindings := sq.bindings |+ (sv2,FLAT (SNOC (unpad dr) ds2)) |>’
+            by (qunabbrev_tac ‘sq’ >> qunabbrev_tac ‘ns’ >>
+                fs[normalise_queues_qpush,DRESTRICT_normalise_queues,
+                   FLOOKUP_normalise_queues_FUPDATE] >>
+                Cases_on ‘sp = sp2’ >> fs[] >-
+                  (fs[APPEND_EQ_CONS] >> rveq >> fs[] >>
+                   fs[qpush_def,SNOC_APPEND,FUPDATE_EQ] >>
+                   rw[normalise_queues_FUPDATE_FUPDATE] >>
+                   rw[normalise_queues_FUPDATE_NONEMPTY]) >>
+                fs[qpush_def] >> rveq >> fs[FUPDATE_COMMUTES] >>
+                simp[SimpR“$=”,Once normalise_queues_FUPDATE_NONEMPTY]) >>
+          first_x_assum SUBST1_TAC >>
+          metis_tac[trans_rules])
+      >- (qmatch_goalsub_abbrev_tac ‘trans _ (NEndpoint c s0 e) _ (NEndpoint c s1 e)’ >>
+          ‘s1 = s0 with queues := qpush s0.queues sp d’
+            by (qunabbrev_tac ‘s0’ >> qunabbrev_tac ‘s1’ >> rw[]) >>
+          rw[] >> metis_tac[trans_rules]))
+  (* LReceive/LTau (Receive intermediate)  *)
+  >- (rename [‘NEndpoint c (s with queues := _) (Receive sp2 sv2 ds2 e)’,
+              ‘LReceive sp d c’,‘qlk s.queues sp2 = dr::tl’] >>
+      qexists_tac ‘NEndpoint c (s with queues := normalise_queues(qpush (s.queues |+ (sp2,tl)) sp d))
+                               (Receive sp2 sv2 (SNOC (unpad dr) ds2) e)’ >>
+      rw[]
+      >- (qmatch_goalsub_abbrev_tac ‘trans _ (NEndpoint _ sq (Receive _ _ _ _)) _
+                                             (NEndpoint _ ns _)’ >>
+          ‘∃tln. qlk sq.queues sp2 = dr::tln’
+            by (qunabbrev_tac ‘sq’ >>
+                fs[qlk_def,fget_def,qpush_def,finite_mapTheory.FLOOKUP_UPDATE] >>
+                Cases_on ‘sp = sp2’ >> Cases_on ‘FLOOKUP s.queues sp2’ >>
+                fs[] >> metis_tac[]) >>
+          ‘ns = sq with
+                <|queues := normalise_queues(sq.queues |+ (sp2,tln))|>’
+            by (qunabbrev_tac ‘sq’ >> qunabbrev_tac ‘ns’ >>
+                fs[qpush_def,qlk_def,fget_def,finite_mapTheory.FLOOKUP_UPDATE] >>
+                Cases_on ‘sp = sp2’ >> fs[]
+                >- (rfs[] >> rw[listTheory.SNOC_APPEND] >> rw[normalise_queues_FUPDATE_NONEMPTY])
+                >- (rw[finite_mapTheory.FUPDATE_COMMUTES,normalise_queues_FUPDATE_NONEMPTY])) >>
+          first_x_assum SUBST1_TAC >>
+          metis_tac[trans_rules])
+      >- (qmatch_goalsub_abbrev_tac ‘trans _ (NEndpoint _ s0 _) _ (NEndpoint _ s1 _)’ >>
+          ‘s1 = s0 with queues := qpush s0.queues sp d’
+            by (qunabbrev_tac ‘s0’ >> qunabbrev_tac ‘s1’ >> rw[]) >>
+          rw[] >> metis_tac[trans_rules]))
+  (* LReceive/LTau (IfThen true) *)
+  >- (rename [‘NEndpoint c (s with queues := qpush s.queues sp d) (IfThen cv e _)’] >>
+      qexists_tac ‘NEndpoint c (s with queues := qpush s.queues sp d) e’ >>
+      rw[]
+      >- (qmatch_goalsub_abbrev_tac ‘NEndpoint c sq’ >>
+          ‘s.bindings = sq.bindings’
+            by simp[Abbr ‘sq’] >>
+          rw[] >>
+          metis_tac[trans_rules])
+      >- metis_tac[trans_rules])
+  (* LReceive/LTau (IfThen false) *)
+  >- (rename [‘NEndpoint c (s with queues := qpush s.queues sp d) (IfThen cv _ e)’] >>
+      qexists_tac ‘NEndpoint c (s with queues := qpush s.queues sp d) e’ >>
+      rw[]
+      >- (qmatch_goalsub_abbrev_tac ‘NEndpoint c sq’ >>
+          ‘s.bindings = sq.bindings’
+            by simp[Abbr ‘sq’] >>
+          rw[] >>
+          metis_tac[trans_rules])
+      >- metis_tac[trans_rules])
+  (* LReceive/LTau (Let statement) *)
+  >- (rename [‘NEndpoint c (s with queues := _) (Let _ _ _ e)’] >>
+      qmatch_goalsub_abbrev_tac ‘s with queues := nq’ >>
+      qmatch_goalsub_abbrev_tac ‘s with bindings := nb’ >>
+      qexists_tac ‘NEndpoint c (s with <|bindings := nb; queues := nq|>) e’ >>
+      rw[]
+      >- (qabbrev_tac ‘IS = s with queues := nq’ >>
+          ‘<|bindings := nb; queues := nq|> = IS with bindings := nb’
+            by simp[Abbr ‘IS’] >>
+          first_x_assum SUBST1_TAC >>
+          qunabbrev_tac ‘nb’ >>
+          ‘s.bindings = IS.bindings’
+            by simp[Abbr ‘IS’] >>
+          first_x_assum SUBST1_TAC >>
+          irule (el 10 (CONJUNCTS trans_rules)) >>
+          simp[Abbr ‘IS’])
+      >- (qabbrev_tac ‘IS = s with bindings := nb’ >>
+          ‘<|bindings := nb; queues := nq|> = IS with queues := nq’
+            by simp[Abbr ‘IS’] >>
+          first_x_assum SUBST1_TAC >>
+          qunabbrev_tac ‘nq’ >>
+          ‘s.queues = IS.queues’
+            by simp[Abbr ‘IS’] >>
+          first_x_assum SUBST1_TAC >>
+          metis_tac[trans_rules]))
+  (* LTau (Internal Comms TO RIGHT) / Parallel Embedded Behaviour (ON LEFT) *)
+  >- (rename [‘net_wf (NPar N1a N1b)’,
+              ‘trans conf (NPar N2Aa N2Ab) _ _ ∧
+               trans conf (NPar N2Ba N1b) _ _’] >>
+      last_x_assum (qspecl_then [‘LB’,‘N2Ba’] assume_tac) >>
+      ‘net_wf N1a’
+        by fs[net_wf_def] >>
+      fs[] >> rfs[] >>
+      first_x_assum (K ALL_TAC) >>
+      ‘LSend p1 d p2 ≠ LB’
+        by (Cases_on ‘LB’ >> fs[wf_label_def] >>
+            rename [‘¬net_has_node (NPar N1a N1b) nint’,
+                    ‘trans conf N1a (LSend p1 d p2) N2Aa’,
+                    ‘trans conf N1b (LReceive p1 d p2) N2Ab’] >>
+            ‘p2 ≠ nint’
+              suffices_by rw[] >>
+            CCONTR_TAC >>
+            ‘net_has_node (NPar N1a N1b) nint’
+              by (‘net_has_node N1b nint’
+                    suffices_by fs[net_has_node_def] >>
+                  metis_tac[trans_receive_cond])) >>
+      fs[] >> first_x_assum (K ALL_TAC) >>
+      ‘wf_label N1a LB’
+        by (Cases_on ‘LB’ >> fs[wf_label_def,net_has_node_def]) >>
+      fs[] >> first_x_assum (K ALL_TAC) >>
+      ‘wf_label N1a (LSend p1 d p2)’
+        by (rw[wf_label_def] >>
+            ‘net_has_node N1b p2’
+              suffices_by (metis_tac[net_wf_def,
+                                     DISJOINT_SYM,
+                                     DISJOINT_ALT,
+                                     IN_APP]) >>
+            metis_tac[trans_receive_cond]) >>
+      fs[] >> first_x_assum (K ALL_TAC) >>
+      rename [‘trans conf N2Aa LB N3’,
+              ‘trans conf N2Ba (LSend p1 d p2) N3’] >>
+      qexists_tac ‘NPar N3 N2Ab’ >>
+      metis_tac[trans_rules])
+  (* LTau (Internal Comms TO RIGHT) / Parallel Embedded Behaviour (ON RIGHT) *)
+  >- (rename [‘net_wf (NPar N1a N1b)’,
+              ‘trans conf (NPar N2Aa N2Ab) _ _ ∧
+               trans conf (NPar N1a N2Bb) _ _’] >>
+      first_x_assum (qspecl_then [‘LB’,‘N2Bb’] assume_tac) >>
+      ‘net_wf N1b’
+        by fs[net_wf_def] >>
+      fs[] >> rfs[] >>
+      first_x_assum (K ALL_TAC) >>
+      ‘∀ds. LReceive p1 ds p2 ≠ LB’
+        by (Cases_on ‘LB’ >> fs[wf_label_def] >>
+            rename [‘¬net_has_node (NPar N1a N1b) nint’,
+                    ‘trans conf N1a (LSend p1 d p2) N2Aa’,
+                    ‘trans conf N1b (LReceive p1 d p2) N2Ab’] >>
+            ‘p1 ≠ nint’
+              suffices_by rw[] >>
+            CCONTR_TAC >>
+            fs[] >>
+            ‘net_has_node (NPar N1a N1b) nint’
+              by (‘net_has_node N1a nint’
+                    suffices_by fs[net_has_node_def] >>
+                  metis_tac[trans_send_cond])) >>
+      fs[] >> first_x_assum (K ALL_TAC) >>
+      ‘wf_label N1b LB’
+        by (Cases_on ‘LB’ >> fs[wf_label_def,net_has_node_def]) >>
+      fs[] >> first_x_assum (K ALL_TAC) >>
+      ‘wf_label N1b (LReceive p1 d p2)’
+        by (rw[wf_label_def] >>
+            ‘net_has_node N1a p1’
+              suffices_by (metis_tac[net_wf_def,
+                                     DISJOINT_SYM,
+                                     DISJOINT_ALT,
+                                     IN_APP]) >>
+            metis_tac[trans_send_cond]) >>
+      fs[] >> first_x_assum (K ALL_TAC) >>
+      rename [‘trans conf N2Ab LB N3’,
+              ‘trans conf N2Bb (LReceive p1 d p2) N3’] >>
+      qexists_tac ‘NPar N2Aa N3’ >>
+      metis_tac[trans_rules])
+  (* LTau (Internal Comms TO LEFT) / Parallel Embedded Behaviour (ON LEFT) *)
+  >- (rename [‘net_wf (NPar N1a N1b)’,
+              ‘trans conf (NPar N2Aa N2Ab) _ _ ∧
+               trans conf (NPar N2Ba N1b) _ _’] >>
+      last_x_assum (qspecl_then [‘LB’,‘N2Ba’] assume_tac) >>
+      ‘net_wf N1a’
+        by fs[net_wf_def] >>
+      fs[] >> rfs[] >>
+      first_x_assum (K ALL_TAC) >>
+      ‘∀ds. LReceive p1 ds p2 ≠ LB’
+        by (Cases_on ‘LB’ >> fs[wf_label_def] >>
+            rename [‘¬net_has_node (NPar N1a N1b) nint’,
+                    ‘trans conf N1a (LReceive p1 d p2) N2Aa’,
+                    ‘trans conf N1b (LSend p1 d p2) N2Ab’] >>
+            ‘p1 ≠ nint’
+              suffices_by rw[] >>
+            CCONTR_TAC >>
+            fs[] >>
+            ‘net_has_node (NPar N1a N1b) nint’
+              by (‘net_has_node N1b nint’
+                    suffices_by fs[net_has_node_def] >>
+                  metis_tac[trans_send_cond])) >>
+      fs[] >> first_x_assum (K ALL_TAC) >>
+      ‘wf_label N1a LB’
+        by (Cases_on ‘LB’ >> fs[wf_label_def,net_has_node_def]) >>
+      fs[] >> first_x_assum (K ALL_TAC) >>
+      ‘wf_label N1a (LReceive p1 d p2)’
+        by (rw[wf_label_def] >>
+            ‘net_has_node N1b p1’
+              suffices_by (metis_tac[net_wf_def,
+                                     DISJOINT_SYM,
+                                     DISJOINT_ALT,
+                                     IN_APP]) >>
+            metis_tac[trans_send_cond]) >>
+      fs[] >> first_x_assum (K ALL_TAC) >>
+      rename [‘trans conf N2Aa LB N3’,
+              ‘trans conf N2Ba (LReceive p1 d p2) N3’] >>
+      qexists_tac ‘NPar N3 N2Ab’ >>
+      metis_tac[trans_rules])
+  (* LTau (Internal Comms TO LEFT) / Other Behaviour (ON RIGHT) *)
+  >- (rename [‘net_wf (NPar N1a N1b)’,
+              ‘trans conf (NPar N2Aa N2Ab) _ _ ∧
+               trans conf (NPar N1a N2Bb) _ _’] >>
+      first_x_assum (qspecl_then [‘LB’,‘N2Bb’] assume_tac) >>
+      ‘net_wf N1b’
+        by fs[net_wf_def] >>
+      fs[] >> rfs[] >>
+      first_x_assum (K ALL_TAC) >>
+      ‘LSend p1 d p2 ≠ LB’
+        by (Cases_on ‘LB’ >> fs[wf_label_def] >>
+            rename [‘¬net_has_node (NPar N1a N1b) nint’,
+                    ‘trans conf N1a (LReceive p1 d p2) N2Aa’,
+                    ‘trans conf N1b (LSend p1 d p2) N2Ab’] >>
+            ‘p2 ≠ nint’
+              suffices_by rw[] >>
+            CCONTR_TAC >>
+            fs[] >>
+            ‘net_has_node (NPar N1a N1b) nint’
+              by (‘net_has_node N1a nint’
+                    suffices_by fs[net_has_node_def] >>
+                  metis_tac[trans_receive_cond])) >>
+      fs[] >> first_x_assum (K ALL_TAC) >>
+      ‘wf_label N1b LB’
+        by (Cases_on ‘LB’ >> fs[wf_label_def,net_has_node_def]) >>
+      fs[] >> first_x_assum (K ALL_TAC) >>
+      ‘wf_label N1b (LSend p1 d p2)’
+        by (rw[wf_label_def] >>
+            ‘net_has_node N1a p2’
+              suffices_by (metis_tac[net_wf_def,
+                                     DISJOINT_SYM,
+                                     DISJOINT_ALT,
+                                     IN_APP]) >>
+            metis_tac[trans_receive_cond]) >>
+      fs[] >> first_x_assum (K ALL_TAC) >>
+      rename [‘trans conf N2Ab LB N3’,
+              ‘trans conf N2Bb (LSend p1 d p2) N3’] >>
+      qexists_tac ‘NPar N2Aa N3’ >>
+      metis_tac[trans_rules])
+  (* LReceive/LTau (Receive Final) *)
+  >- (rename [‘NEndpoint c (s with queues := _) (Receive sp2 sv2 ds2 e)’,
+              ‘LReceive sp d c’] >>
+      qmatch_goalsub_abbrev_tac ‘<|bindings := fb; queues := bfq |>’ >>
+      qexists_tac ‘NEndpoint c <|bindings := fb; queues := normalise_queues(qpush bfq sp d)|> e’ >>
+      rw[]
+      >- (qmatch_goalsub_abbrev_tac ‘trans _ (NEndpoint c s0 e) _ (NEndpoint c s1 e)’ >>
+          ‘s1 = s0 with queues := qpush s0.queues sp d’
+            by (qunabbrev_tac ‘s0’ >> qunabbrev_tac ‘s1’ >> rw[Abbr ‘bfq’]) >>
+          rw[] >> metis_tac[trans_rules])
+      >- (qunabbrev_tac ‘bfq’ >> qunabbrev_tac ‘fb’ >>
+          qmatch_goalsub_abbrev_tac ‘trans _ (NEndpoint _ sq (Receive _ _ _ _)) _
+                                             (NEndpoint _ ns _)’ >>
+          rename1 ‘qlk s.queues sp2 = dr::tl’ >>
+          ‘∃tln. qlk sq.queues sp2 = dr::tln’
+            by (qunabbrev_tac ‘sq’ >>
+                fs[qlk_def,fget_def,qpush_def,finite_mapTheory.FLOOKUP_UPDATE] >>
+                Cases_on ‘sp = sp2’ >> Cases_on ‘FLOOKUP s.queues sp2’ >>
+                fs[] >> metis_tac[]) >>
+          ‘ns = sq with
+                <|queues := normalise_queues(sq.queues |+ (sp2,tln));
+                  bindings := sq.bindings |+ (sv2,FLAT (SNOC (unpad dr) ds2)) |>’
+            by (qunabbrev_tac ‘sq’ >> qunabbrev_tac ‘ns’ >>
+                fs[qpush_def,qlk_def,fget_def,finite_mapTheory.FLOOKUP_UPDATE] >>
+                Cases_on ‘sp = sp2’ >> fs[]
+                >- (rfs[] >> rw[listTheory.SNOC_APPEND] >> rw[normalise_queues_FUPDATE_NONEMPTY])
+                >- (rw[finite_mapTheory.FUPDATE_COMMUTES,normalise_queues_FUPDATE_NONEMPTY])) >>
+          first_x_assum SUBST1_TAC >>
+          metis_tac[trans_rules]))
+  (* LTau (Receive intermediate)/LReceive  *)
+  >- (rename [‘NEndpoint c (s with queues := _) (Receive sp2 sv2 (SNOC (unpad dr) ds2) e)’,
+              ‘LReceive sp d c’,‘qlk s.queues sp2 = dr::tl’] >>
+      qexists_tac ‘NEndpoint c (s with queues := normalise_queues(qpush (s.queues |+ (sp2,tl)) sp d))
+                               (Receive sp2 sv2 (SNOC (unpad dr) ds2) e)’ >>
+      rw[]
+      >- (qmatch_goalsub_abbrev_tac ‘trans _ (NEndpoint _ s0 _) _ (NEndpoint _ s1 _)’ >>
+          ‘s1 = s0 with queues := qpush s0.queues sp d’
+            by (qunabbrev_tac ‘s0’ >> qunabbrev_tac ‘s1’ >> rw[]) >>
+          rw[] >> metis_tac[trans_rules])
+      >- (qmatch_goalsub_abbrev_tac ‘trans _ (NEndpoint _ sq (Receive _ _ _ _)) _
+                                             (NEndpoint _ ns _)’ >>
+          ‘∃tln. qlk sq.queues sp2 = dr::tln’
+            by (qunabbrev_tac ‘sq’ >>
+                fs[qlk_def,fget_def,qpush_def,finite_mapTheory.FLOOKUP_UPDATE] >>
+                Cases_on ‘sp = sp2’ >> Cases_on ‘FLOOKUP s.queues sp2’ >>
+                fs[] >> metis_tac[]) >>
+          ‘ns = sq with
+                <|queues := normalise_queues(sq.queues |+ (sp2,tln))|>’
+            by (qunabbrev_tac ‘sq’ >> qunabbrev_tac ‘ns’ >>
+                fs[qpush_def,qlk_def,fget_def,finite_mapTheory.FLOOKUP_UPDATE] >>
+                Cases_on ‘sp = sp2’ >> fs[]
+                >- (rfs[] >> rw[listTheory.SNOC_APPEND] >> rw[normalise_queues_FUPDATE_NONEMPTY])
+                >- (rw[finite_mapTheory.FUPDATE_COMMUTES,normalise_queues_FUPDATE_NONEMPTY])) >>
+          first_x_assum SUBST1_TAC >>
+          metis_tac[trans_rules]))
+  (* LTau (IfThen true)/LReceive *)
+  >- (rename [‘NEndpoint c (s with queues := qpush s.queues sp d) (IfThen cv e _)’] >>
+      qexists_tac ‘NEndpoint c (s with queues := qpush s.queues sp d) e’ >>
+      rw[]
+      >- metis_tac[trans_rules]
+      >- (qmatch_goalsub_abbrev_tac ‘NEndpoint c sq’ >>
+          ‘s.bindings = sq.bindings’
+            by simp[Abbr ‘sq’] >>
+          rw[] >>
+          metis_tac[trans_rules]))
+  (* LTau (IfThen false)/LReceive *)
+  >- (rename [‘NEndpoint c (s with queues := qpush s.queues sp d) (IfThen cv _ e)’] >>
+      qexists_tac ‘NEndpoint c (s with queues := qpush s.queues sp d) e’ >>
+      rw[]
+      >- metis_tac[trans_rules]
+      >- (qmatch_goalsub_abbrev_tac ‘NEndpoint c sq’ >>
+          ‘s.bindings = sq.bindings’
+            by simp[Abbr ‘sq’] >>
+          rw[] >>
+          metis_tac[trans_rules]))
+  (* LTau (Let statement)/LReceive *)
+  >- (rename [‘NEndpoint c (s with queues := _) (Let _ _ _ e)’] >>
+      qmatch_goalsub_abbrev_tac ‘s with queues := nq’ >>
+      qmatch_goalsub_abbrev_tac ‘s with bindings := nb’ >>
+      qexists_tac ‘NEndpoint c (s with <|bindings := nb; queues := nq|>) e’ >>
+      rw[]
+      >- (qabbrev_tac ‘IS = s with bindings := nb’ >>
+          ‘<|bindings := nb; queues := nq|> = IS with queues := nq’
+            by simp[Abbr ‘IS’] >>
+          first_x_assum SUBST1_TAC >>
+          qunabbrev_tac ‘nq’ >>
+          ‘s.queues = IS.queues’
+            by simp[Abbr ‘IS’] >>
+          first_x_assum SUBST1_TAC >>
+          metis_tac[trans_rules])
+      >- (qabbrev_tac ‘IS = s with queues := nq’ >>
+          ‘<|bindings := nb; queues := nq|> = IS with bindings := nb’
+            by simp[Abbr ‘IS’] >>
+          first_x_assum SUBST1_TAC >>
+          qunabbrev_tac ‘nb’ >>
+          ‘s.bindings = IS.bindings’
+            by simp[Abbr ‘IS’] >>
+          first_x_assum SUBST1_TAC >>
+          irule (el 10 (CONJUNCTS trans_rules)) >>
+          simp[Abbr ‘IS’]))
+  (* Parallel Embedded Behaviour (ON LEFT)/LTau (Internal Comms TO RIGHT) /  *)
+  >- (rename [‘net_wf (NPar N1a N1b)’,
+              ‘trans conf (NPar N2Aa N1b)  _ _ ∧
+               trans conf (NPar N2Ba N2Bb) _ _’] >>
+      last_x_assum (qspecl_then [‘LSend p1 d p2’,‘N2Ba’] assume_tac) >>
+      ‘net_wf N1a’
+        by fs[net_wf_def] >>
+      fs[] >> rfs[] >>
+      first_x_assum (K ALL_TAC) >>
+      ‘LA ≠ LSend p1 d p2’
+        by (Cases_on ‘LA’ >> fs[wf_label_def] >>
+            rename [‘¬net_has_node (NPar N1a N1b) nint’,
+                    ‘trans conf N1a (LSend p1 d p2) N2Aa’,
+                    ‘trans conf N1b (LReceive p1 d p2) N2Ab’] >>
+            ‘p2 ≠ nint’
+              suffices_by rw[] >>
+            CCONTR_TAC >>
+            ‘net_has_node (NPar N1a N1b) nint’
+              by (‘net_has_node N1b nint’
+                    suffices_by fs[net_has_node_def] >>
+                  metis_tac[trans_receive_cond])) >>
+      fs[] >> first_x_assum (K ALL_TAC) >>
+      ‘wf_label N1a LA’
+        by (Cases_on ‘LA’ >> fs[wf_label_def,net_has_node_def]) >>
+      fs[] >> first_x_assum (K ALL_TAC) >>
+      ‘wf_label N1a (LSend p1 d p2)’
+        by (rw[wf_label_def] >>
+            ‘net_has_node N1b p2’
+              suffices_by (metis_tac[net_wf_def,
+                                     DISJOINT_SYM,
+                                     DISJOINT_ALT,
+                                     IN_APP]) >>
+            metis_tac[trans_receive_cond]) >>
+      fs[] >> first_x_assum (K ALL_TAC) >>
+      rename [‘trans conf N2Aa (LSend p1 d p2) N3’,
+              ‘trans conf N2Ba LA N3’] >>
+      qexists_tac ‘NPar N3 N2Bb’ >>
+      metis_tac[trans_rules])
+  (*  Parallel Embedded Behaviour (ON LEFT) / LTau (Internal Comms TO RIGHT) *)
+  >- (rename [‘net_wf (NPar N1a N1b)’,
+              ‘LReceive sp d rp’,
+              ‘trans conf (NPar N2Aa N1b) _ _ ∧
+               trans conf (NPar N2Ba N2Bb) _ _’] >>
+      first_x_assum (qspecl_then [‘LReceive sp d rp’,‘N2Ba’] assume_tac) >>
+      ‘net_wf N1a’
+        by fs[net_wf_def] >>
+      fs[] >> rfs[] >>
+      first_x_assum (K ALL_TAC) >>
+      ‘∀ds. LReceive sp ds rp ≠ LA’
+        by (Cases_on ‘LA’ >> fs[wf_label_def] >>
+            rename [‘¬net_has_node (NPar N1a N1b) nint’,
+                    ‘trans conf N1a (LReceive sp d rp) N2Aa’,
+                    ‘trans conf N1b (LSend sp d rp) N2Ab’] >>
+            DISJ1_TAC >> CCONTR_TAC >> fs[] >>
+            ‘net_has_node (NPar N1a N1b) nint’
+              by (‘net_has_node N1b nint’
+                    suffices_by fs[net_has_node_def] >>
+                  metis_tac[trans_send_cond])) >>
+      fs[] >> first_x_assum (K ALL_TAC) >>
+      ‘wf_label N1a LA’
+        by (Cases_on ‘LA’ >> fs[wf_label_def,net_has_node_def]) >>
+      fs[] >> first_x_assum (K ALL_TAC) >>
+      ‘wf_label N1a (LReceive sp d rp)’
+        by (rw[wf_label_def] >>
+            ‘net_has_node N1b sp’
+              suffices_by (metis_tac[net_wf_def,
+                                     DISJOINT_SYM,
+                                     DISJOINT_ALT,
+                                     IN_APP]) >>
+            metis_tac[trans_send_cond]) >>
+      fs[] >> first_x_assum (K ALL_TAC) >>
+      rename [‘trans conf N2Ba LA N3’,
+              ‘trans conf N2Aa (LReceive sp d rp) N3’] >>
+      qexists_tac ‘NPar N3 N2Bb’ >>
+      metis_tac[trans_rules])
+  (* Parallel Embeded Behaviour (ON LEFT) / Parallel Embedded Behaviour (ON LEFT) *)
+  >- (rename [‘net_wf (NPar N1a N1b)’,
+              ‘trans conf (NPar N2Aa N1b) _ _ ∧
+               trans conf (NPar N2Ba N1b) _ _’] >>
+      last_x_assum (qspecl_then [‘LB’,‘N2Ba’] assume_tac) >>
+      ‘net_wf N1a’
+        by fs[net_wf_def] >>
+      ‘wf_label N1a LA’
+        by (Cases_on ‘LA’ >>
+            fs[wf_label_def,net_has_node_def]) >>
+      ‘wf_label N1a LB’
+        by (Cases_on ‘LB’ >>
+            fs[wf_label_def,net_has_node_def]) >>
+      fs[] >> ntac 3 (pop_assum (K ALL_TAC)) >>
+      qmatch_asmsub_abbrev_tac ‘predA ∧ predB ∧ predC ⇒
+                                ∃N3. trans conf N2Aa LB N3 ∧
+                                     trans conf N2Ba LA N3’ >>
+      qpat_x_assum ‘predA’ assume_tac >>
+      qpat_x_assum ‘predB’ assume_tac >>
+      qpat_x_assum ‘predC’ assume_tac >>
+      fs[] >> ntac 6 (pop_assum (K ALL_TAC)) >>
+      qexists_tac ‘NPar N3 N1b’ >>
+      metis_tac[trans_rules])
+  (* Parallel Embeded Behaviour (ON LEFT) / Parallel Embedded Behaviour (ON RIGHT) *)
+  >- (rename [‘net_wf (NPar N1a N1b)’,
+              ‘trans conf (NPar N2Aa N1b) _ _ ∧
+               trans conf (NPar N1a N2Bb) _ _’] >>
+      qexists_tac ‘NPar N2Aa N2Bb’ >>
+      metis_tac[trans_rules])
+  (* Parallel Embedded Behaviour (ON RIGHT) / LTau (Internal Comms TO RIGHT) *)
+  >- (rename [‘net_wf (NPar N1a N1b)’,
+              ‘LReceive sp d rp’,
+              ‘trans conf (NPar N1a N2Ab) _ _ ∧
+               trans conf (NPar N2Ba N2Bb) _ _’] >>
+      last_x_assum (qspecl_then [‘LReceive sp d rp’,‘N2Bb’] assume_tac) >>
+      ‘net_wf N1b’
+        by fs[net_wf_def] >>
+      fs[] >> rfs[] >>
+      first_x_assum (K ALL_TAC) >>
+      ‘∀ds. LReceive sp ds rp ≠ LA’
+        by (Cases_on ‘LA’ >> fs[wf_label_def] >>
+            rename [‘¬net_has_node (NPar N1a N1b) nint’] >>
+            DISJ1_TAC >>
+            CCONTR_TAC >>
+            fs[] >>
+            ‘net_has_node (NPar N1a N1b) nint’
+              by (‘net_has_node N1a nint’
+                    suffices_by fs[net_has_node_def] >>
+                  metis_tac[trans_send_cond])) >>
+      fs[] >> first_x_assum (K ALL_TAC) >>
+      ‘wf_label N1b LA’
+        by (Cases_on ‘LA’ >> fs[wf_label_def,net_has_node_def]) >>
+      fs[] >> first_x_assum (K ALL_TAC) >>
+      ‘wf_label N1b (LReceive sp d rp)’
+        by (rw[wf_label_def] >>
+            ‘net_has_node N1a sp’
+              suffices_by (metis_tac[net_wf_def,
+                                     DISJOINT_SYM,
+                                     DISJOINT_ALT,
+                                     IN_APP]) >>
+            metis_tac[trans_send_cond]) >>
+      fs[] >> first_x_assum (K ALL_TAC) >>
+      rename [‘trans conf N2Ab (LReceive sp d rp) N3’,
+              ‘trans conf N2Bb  LA N3’] >>
+      qexists_tac ‘NPar N2Ba N3’ >>
+      metis_tac[trans_rules])
+  (* Parallel Embedded Behaviour (ON RIGHT) / LTau (Internal Comms TO LEFT) *)
+  >- (rename [‘net_wf (NPar N1a N1b)’,
+          ‘LReceive sp d rp’,
+              ‘trans conf (NPar N1a N2Ab) _ _ ∧
+               trans conf (NPar N2Ba N2Bb) _ _’] >>
+      first_x_assum (qspecl_then [‘LSend sp d rp’,‘N2Bb’] assume_tac) >>
+      ‘net_wf N1b’
+        by fs[net_wf_def] >>
+      fs[] >> rfs[] >>
+      first_x_assum (K ALL_TAC) >>
+      ‘LA ≠ LSend sp d rp’
+        by (Cases_on ‘LA’ >> fs[wf_label_def] >>
+            rename [‘¬net_has_node (NPar N1a N1b) nint’] >>
+            ‘rp ≠ nint’
+              suffices_by rw[] >>
+            CCONTR_TAC >>
+            ‘net_has_node (NPar N1a N1b) nint’
+              by (‘net_has_node N1a nint’
+                    suffices_by fs[net_has_node_def] >>
+                  metis_tac[trans_receive_cond])) >>
+      fs[] >> first_x_assum (K ALL_TAC) >>
+      ‘wf_label N1b LA’
+        by (Cases_on ‘LA’ >> fs[wf_label_def,net_has_node_def]) >>
+      fs[] >> first_x_assum (K ALL_TAC) >>
+      ‘wf_label N1b (LSend sp d rp)’
+        by (rw[wf_label_def] >>
+            ‘net_has_node N1a rp’
+              suffices_by (metis_tac[net_wf_def,
+                                     DISJOINT_SYM,
+                                     DISJOINT_ALT,
+                                     IN_APP]) >>
+            metis_tac[trans_receive_cond]) >>
+      fs[] >> first_x_assum (K ALL_TAC) >>
+      rename [‘trans conf N2Ab (LSend sp d rp) N3’,
+              ‘trans conf N2Bb LA N3’] >>
+      qexists_tac ‘NPar N2Ba N3’ >>
+      metis_tac[trans_rules])
+  (* Parallel Embedded Behaviour (ON RIGHT) / Parallel Embedded Behaviour (ON LEFT) *)
+  >- (rename [‘net_wf (NPar N1a N1b)’,
+              ‘trans conf (NPar N1a N2Ab) _ _ ∧
+               trans conf (NPar N2Ba N1b) _ _’] >>
+      qexists_tac ‘NPar N2Ba N2Ab’ >>
+      metis_tac[trans_rules])
+  (* Parallel Embedded Behaviour (ON RIGHT) / Parallel Embedded Behaviour (ON RIGHT) *)
+  >- (rename [‘net_wf (NPar N1a N1b)’,
+              ‘trans conf (NPar N1a N2Ab) _ _ ∧
+               trans conf (NPar N1a N2Bb) _ _’] >>
+      last_x_assum (qspecl_then [‘LB’,‘N2Bb’] assume_tac) >>
+      ‘net_wf N1b’
+        by fs[net_wf_def] >>
+      ‘wf_label N1b LA’
+        by (Cases_on ‘LA’ >>
+            fs[wf_label_def,net_has_node_def]) >>
+      ‘wf_label N1b LB’
+        by (Cases_on ‘LB’ >>
+            fs[wf_label_def,net_has_node_def]) >>
+      fs[] >> ntac 3 (pop_assum (K ALL_TAC)) >>
+      qmatch_asmsub_abbrev_tac ‘predA ∧ predB ∧ predC ⇒
+                                ∃N3. trans conf N2Ab LB N3 ∧
+                                     trans conf N2Bb LA N3’ >>
+      qpat_x_assum ‘predA’ assume_tac >>
+      qpat_x_assum ‘predB’ assume_tac >>
+      qpat_x_assum ‘predC’ assume_tac >>
+      fs[] >> ntac 6 (pop_assum (K ALL_TAC)) >>
+      qexists_tac ‘NPar N1a N3’ >>
+      metis_tac[trans_rules])
+QED
+
+(* Confluence Results for identical Labels *)
+(* -- Functional nature for non-tau labels *)
+Theorem trans_notau_functional:
+  ∀conf N1 N2A N2B L.
+    L ≠ LTau ∧
+    trans conf N1 L N2A ∧
+    trans conf N1 L N2B ∧
+    net_wf N1 ⇒
+    N2A = N2B
+Proof
+  Cases_on ‘L’ >> fs[] >>
+  Induct_on ‘trans’ >> rw[]
+  >- (fs[Once trans_cases] >>
+      rename1 ‘LENGTH d2 > n + conf.payload_size’ >>
+      ‘LENGTH d2 ≤ n + conf.payload_size’
+        by fs[pad_def] >>
+      fs[])
+  >- (fs[Once trans_cases] >>
+      rename1 ‘LENGTH d2 ≤ n + conf.payload_size’ >>
+      ‘LENGTH d2 > n + conf.payload_size’
+        by fs[pad_def] >>
+      fs[])
+  >- (fs[net_wf_def,DISJOINT_DEF,
+         EXTENSION,IN_DEF] >>
+      rename [‘LSend sp d rp’,‘NPar N1A N1B’] >>
+      ‘¬(∃N1BS. trans conf N1B (LSend sp d rp) N1BS)’
+        by metis_tac[trans_send_cond] >>
+      fs[] >>
+      ntac 2 (last_x_assum assume_tac) >>
+      first_x_assum (assume_tac o REWRITE_RULE [Once trans_cases]) >>
+      rfs[])
+  >- (fs[net_wf_def,DISJOINT_DEF,
+         EXTENSION,IN_DEF] >>
+      rename [‘LSend sp d rp’,‘NPar N1A N1B’] >>
+      ‘¬(∃N1AS. trans conf N1A (LSend sp d rp) N1AS)’
+        by metis_tac[trans_send_cond] >>
+      fs[] >>
+      ntac 2 (last_x_assum assume_tac) >>
+      first_x_assum (assume_tac o REWRITE_RULE [Once trans_cases]) >>
+      rfs[])
+  >- fs[Once trans_cases]
+  >- (fs[net_wf_def,DISJOINT_DEF,
+         EXTENSION,IN_DEF] >>
+      rename [‘LReceive sp d rp’,‘NPar N1A N1B’] >>
+      ‘¬(∃N1BR. trans conf N1B (LReceive sp d rp) N1BR)’
+        by metis_tac[trans_receive_cond] >>
+      fs[] >>
+      ntac 2 (last_x_assum assume_tac) >>
+      first_x_assum (assume_tac o REWRITE_RULE [Once trans_cases]) >>
+      rfs[])
+  >- (fs[net_wf_def,DISJOINT_DEF,
+         EXTENSION,IN_DEF] >>
+      rename [‘LReceive sp d rp’,‘NPar N1A N1B’] >>
+      ‘¬(∃N1AR. trans conf N1A (LReceive sp d rp) N1AR)’
+        by metis_tac[trans_receive_cond] >>
+      fs[] >>
+      ntac 2 (last_x_assum assume_tac) >>
+      first_x_assum (assume_tac o REWRITE_RULE [Once trans_cases]) >>
+      rfs[])
+QED
+
+(* -- Confluence: Identical tau labels *)
+Theorem trans_samelab_tau_difout_diamond[local]:
+  ∀N1 N2A N2B.
+    net_wf N1 ∧
+    N2A ≠ N2B ∧
+    trans conf N1 LTau N2A ∧
+    trans conf N1 LTau N2B ⇒
+    ∃N3.
+      trans conf N2A LTau N3 ∧
+      trans conf N2B LTau N3
+Proof
+        Induct_on ‘N1’
+  (* NNil Case *)
+  >- (rw[] >> fs[Once trans_cases])
+  (* NPar Case *)
+  >- (rw[] >> rename1 ‘net_wf (NPar N1a N1b)’ >>
+      qpat_x_assum ‘trans _ (NPar _ _) _ N2A’
+                  (fn x => strip_assume_tac(REWRITE_RULE [Once trans_cases] x)) >>
+      fs[] >> rw[] >> fs[] >>
+      qpat_x_assum ‘trans _ (NPar _ _) _ _’
+                  (fn x => strip_assume_tac(REWRITE_RULE [Once trans_cases] x)) >>
+      fs[] >> rw[] >> fs[]
+      (* (FIRST DIFF) Internal Comms (TO RIGHT) / Internal Comms (TO RIGHT) *)
+      >- (rename [‘trans conf (NPar N2Aa N2Ab) LTau _ ∧
+                     trans conf (NPar N2Ba N2Bb) LTau _’,
+                    ‘net_wf (NPar N1a N1b)’,
+                    ‘trans conf N1a (LSend spA dA rpA) N2Aa’,
+                    ‘trans conf N1a (LSend spB dB rpB) N2Ba’] >>
+          ‘∃N3a.
+            trans conf N2Aa (LSend spB dB rpB) N3a ∧
+            trans conf N2Ba (LSend spA dA rpA) N3a’
+            by (irule trans_diff_diamond >>
+                rw[compat_labels_def]
+                >- (CCONTR_TAC >>
+                    ‘N2Aa = N2Ba’
+                      suffices_by rw[] >>
+                    irule trans_notau_functional >>
+                    MAP_EVERY qexists_tac [‘LSend spB dB rpB’,
+                                            ‘N1a’,‘conf’] >>
+                    fs[net_wf_def])
+                >- (qexists_tac ‘N1a’ >>
+                    fs[net_wf_def,wf_label_def,compat_labels_def] >>
+                    ‘net_has_node N1b rpA ∧ net_has_node N1b rpB’
+                      suffices_by metis_tac[DISJOINT_SYM,
+                                            DISJOINT_ALT,
+                                            IN_APP] >>
+                    metis_tac[trans_receive_cond])) >>
+          ‘∃N3b.
+            trans conf N2Ab (LReceive spB dB rpB) N3b ∧
+            trans conf N2Bb (LReceive spA dA rpA) N3b’
+            by (irule trans_diff_diamond >>
+                rw[]
+                >- (CCONTR_TAC >>
+                    ‘N2Aa = N2Ba’
+                      suffices_by rw[] >>
+                    irule trans_notau_functional >>
+                    MAP_EVERY qexists_tac [‘LSend spB dB rpB’,
+                                            ‘N1a’,‘conf’] >>
+                    fs[net_wf_def])
+                >- metis_tac[send_gen_compat,net_wf_def]
+                >- (qexists_tac ‘N1b’ >>
+                    fs[net_wf_def,wf_label_def,compat_labels_def] >>
+                    ‘net_has_node N1a spA ∧ net_has_node N1a spB’
+                      suffices_by metis_tac[DISJOINT_SYM,
+                                            DISJOINT_ALT,
+                                            IN_APP] >>
+                    metis_tac[trans_send_cond])) >>
+          qexists_tac ‘NPar N3a N3b’ >>
+          metis_tac[trans_rules])
+      (* (SECOND DIFF) Internal Comms (TO RIGHT) / Internal Comms (TO RIGHT) *)
+      >- (rename [‘trans conf (NPar N2Aa N2Ab) LTau _ ∧
+                   trans conf (NPar N2Ba N2Bb) LTau _’,
+                  ‘net_wf (NPar N1a N1b)’,
+                  ‘trans conf N1a (LSend spA dA rpA) N2Aa’,
+                  ‘trans conf N1a (LSend spB dB rpB) N2Ba’] >>
+          ‘∃N3a.
+            trans conf N2Aa (LSend spB dB rpB) N3a ∧
+            trans conf N2Ba (LSend spA dA rpA) N3a’
+            by (irule trans_diff_diamond >>
+                rw[compat_labels_def]
+                >- (CCONTR_TAC >>
+                    ‘N2Ab = N2Bb’
+                      suffices_by rw[] >>
+                    irule trans_notau_functional >>
+                    MAP_EVERY qexists_tac [‘LReceive spB dB rpB’,
+                                            ‘N1b’,‘conf’] >>
+                    fs[net_wf_def])
+                >- (qexists_tac ‘N1a’ >>
+                    fs[net_wf_def,wf_label_def,compat_labels_def] >>
+                    ‘net_has_node N1b rpA ∧ net_has_node N1b rpB’
+                      suffices_by metis_tac[DISJOINT_SYM,
+                                            DISJOINT_ALT,
+                                            IN_APP] >>
+                    metis_tac[trans_receive_cond])) >>
+          ‘∃N3b.
+            trans conf N2Ab (LReceive spB dB rpB) N3b ∧
+            trans conf N2Bb (LReceive spA dA rpA) N3b’
+            by (irule trans_diff_diamond >>
+                rw[]
+                >- (CCONTR_TAC >>
+                    ‘N2Ab = N2Bb’
+                      suffices_by rw[] >>
+                    irule trans_notau_functional >>
+                    MAP_EVERY qexists_tac [‘LReceive spB dB rpB’,
+                                            ‘N1b’,‘conf’] >>
+                    fs[net_wf_def])
+                >- metis_tac[send_gen_compat,net_wf_def]
+                >- (qexists_tac ‘N1b’ >>
+                    fs[net_wf_def,wf_label_def,compat_labels_def] >>
+                    ‘net_has_node N1a spA ∧ net_has_node N1a spB’
+                      suffices_by metis_tac[DISJOINT_SYM,
+                                            DISJOINT_ALT,
+                                            IN_APP] >>
+                    metis_tac[trans_send_cond])) >>
+          qexists_tac ‘NPar N3a N3b’ >>
+          metis_tac[trans_rules])
+      (* (FIRST DIFF) Internal Comms (TO RIGHT) / Internal Comms (TO LEFT) *)
+      >- (rename [‘trans conf (NPar N2Aa N2Ab) LTau _ ∧
+                   trans conf (NPar N2Ba N2Bb) LTau _’,
+                  ‘net_wf (NPar N1a N1b)’,
+                  ‘trans conf N1a (LSend spA dA rpA) N2Aa’,
+                  ‘trans conf N1b (LSend spB dB rpB) N2Bb’] >>
+          ‘∃N3a.
+            trans conf N2Aa (LReceive spB dB rpB) N3a ∧
+            trans conf N2Ba (LSend spA dA rpA) N3a’
+            by (irule trans_diff_diamond >>
+                rw[compat_labels_def] >>
+                qexists_tac ‘N1a’ >>
+                fs[net_wf_def,wf_label_def,compat_labels_def] >>
+                ‘net_has_node N1b rpA ∧ net_has_node N1b spB’
+                      suffices_by metis_tac[DISJOINT_SYM,
+                                            DISJOINT_ALT,
+                                            IN_APP] >>
+                metis_tac[trans_send_cond,trans_receive_cond]) >>
+          ‘∃N3b.
+            trans conf N2Ab (LSend spB dB rpB) N3b ∧
+            trans conf N2Bb (LReceive spA dA rpA) N3b’
+            by (irule trans_diff_diamond >>
+                rw[compat_labels_def] >>
+                qexists_tac ‘N1b’ >>
+                fs[net_wf_def,wf_label_def] >>
+                ‘net_has_node N1a spA ∧ net_has_node N1a rpB’
+                  suffices_by metis_tac[DISJOINT_SYM,
+                                        DISJOINT_ALT,
+                                        IN_APP] >>
+                metis_tac[trans_send_cond,trans_receive_cond]) >>
+          qexists_tac ‘NPar N3a N3b’ >>
+          metis_tac[trans_rules])
+      (* (SECOND DIFF) Internal Comms (TO RIGHT) / Internal Comms (TO LEFT) *)
+      >- (rename [‘trans conf (NPar N2Aa N2Ab) LTau _ ∧
+                   trans conf (NPar N2Ba N2Bb) LTau _’,
+                  ‘net_wf (NPar N1a N1b)’,
+                  ‘trans conf N1a (LSend spA dA rpA) N2Aa’,
+                  ‘trans conf N1b (LSend spB dB rpB) N2Bb’] >>
+          ‘∃N3a.
+            trans conf N2Aa (LReceive spB dB rpB) N3a ∧
+            trans conf N2Ba (LSend spA dA rpA) N3a’
+            by (irule trans_diff_diamond >>
+                rw[compat_labels_def] >>
+                qexists_tac ‘N1a’ >>
+                fs[net_wf_def,wf_label_def,compat_labels_def] >>
+                ‘net_has_node N1b rpA ∧ net_has_node N1b spB’
+                      suffices_by metis_tac[DISJOINT_SYM,
+                                            DISJOINT_ALT,
+                                            IN_APP] >>
+                metis_tac[trans_send_cond,trans_receive_cond]) >>
+          ‘∃N3b.
+            trans conf N2Ab (LSend spB dB rpB) N3b ∧
+            trans conf N2Bb (LReceive spA dA rpA) N3b’
+            by (irule trans_diff_diamond >>
+                rw[compat_labels_def] >>
+                qexists_tac ‘N1b’ >>
+                fs[net_wf_def,wf_label_def] >>
+                ‘net_has_node N1a spA ∧ net_has_node N1a rpB’
+                  suffices_by metis_tac[DISJOINT_SYM,
+                                        DISJOINT_ALT,
+                                        IN_APP] >>
+                metis_tac[trans_send_cond,trans_receive_cond]) >>
+          qexists_tac ‘NPar N3a N3b’ >>
+          metis_tac[trans_rules])
+      (* (FIRST DIFF) Internal Comms (TO RIGHT) / Parallel Embedded Behaviour (LEFT) *)
+      >- (rename [‘trans conf (NPar N2Aa N2Ab) LTau _ ∧
+                   trans conf (NPar N2Ba N1b) LTau _’,
+                  ‘net_wf (NPar N1a N1b)’,
+                  ‘trans conf N1a (LSend sp d rp) N2Aa’] >>
+          ‘∃N3a.
+            trans conf N2Aa LTau N3a ∧
+            trans conf N2Ba (LSend sp d rp) N3a’
+            by (irule trans_diff_diamond >>
+                rw[compat_labels_def] >>
+                qexists_tac ‘N1a’ >>
+                fs[net_wf_def,wf_label_def,compat_labels_def] >>
+                ‘net_has_node N1b rp’
+                      suffices_by metis_tac[DISJOINT_SYM,
+                                            DISJOINT_ALT,
+                                            IN_APP] >>
+                metis_tac[trans_receive_cond]) >>
+          qexists_tac ‘NPar N3a N2Ab’ >>
+          metis_tac[trans_rules])
+      (* (SECOND DIFF) Internal Comms (TO RIGHT) / Parallel Embedded Behaviour (LEFT) *)
+      >- (rename [‘trans conf (NPar N2Aa N2Ab) LTau _ ∧
+                   trans conf (NPar N2Ba N1b) LTau _’,
+                  ‘net_wf (NPar N1a N1b)’,
+                  ‘trans conf N1a (LSend sp d rp) N2Aa’] >>
+          ‘∃N3a.
+            trans conf N2Aa LTau N3a ∧
+            trans conf N2Ba (LSend sp d rp) N3a’
+            by (irule trans_diff_diamond >>
+                rw[compat_labels_def] >>
+                qexists_tac ‘N1a’ >>
+                fs[net_wf_def,wf_label_def,compat_labels_def] >>
+                ‘net_has_node N1b rp’
+                      suffices_by metis_tac[DISJOINT_SYM,
+                                            DISJOINT_ALT,
+                                            IN_APP] >>
+                metis_tac[trans_receive_cond]) >>
+          qexists_tac ‘NPar N3a N2Ab’ >>
+          metis_tac[trans_rules])
+      (* (FIRST DIFF) Internal Comms (TO RIGHT) / Parallel Embedded Behaviour (RIGHT) *)
+      >- (rename [‘trans conf (NPar N2Aa N2Ab) LTau _ ∧
+                   trans conf (NPar N1a N2Bb) LTau _’,
+                  ‘net_wf (NPar N1a N1b)’,
+                  ‘trans conf N1a (LSend sp d rp) N2Aa’] >>
+          ‘∃N3b.
+            trans conf N2Ab LTau N3b ∧
+            trans conf N2Bb (LReceive sp d rp) N3b’
+            by (irule trans_diff_diamond >>
+                rw[compat_labels_def] >>
+                qexists_tac ‘N1b’ >>
+                fs[net_wf_def,wf_label_def,compat_labels_def] >>
+                ‘net_has_node N1a sp’
+                      suffices_by metis_tac[DISJOINT_SYM,
+                                            DISJOINT_ALT,
+                                            IN_APP] >>
+                metis_tac[trans_send_cond]) >>
+          qexists_tac ‘NPar N2Aa N3b’ >>
+          metis_tac[trans_rules])
+      (* (SECOND DIFF) Internal Comms (TO RIGHT) / Parallel Embedded Behaviour (LEFT) *)
+      >- (rename [‘trans conf (NPar N2Aa N2Ab) LTau _ ∧
+                   trans conf (NPar N1a N2Bb) LTau _’,
+                  ‘net_wf (NPar N1a N1b)’,
+                  ‘trans conf N1a (LSend sp d rp) N2Aa’] >>
+          ‘∃N3b.
+            trans conf N2Ab LTau N3b ∧
+            trans conf N2Bb (LReceive sp d rp) N3b’
+            by (irule trans_diff_diamond >>
+                rw[compat_labels_def] >>
+                qexists_tac ‘N1b’ >>
+                fs[net_wf_def,wf_label_def,compat_labels_def] >>
+                ‘net_has_node N1a sp’
+                      suffices_by metis_tac[DISJOINT_SYM,
+                                            DISJOINT_ALT,
+                                            IN_APP] >>
+                metis_tac[trans_send_cond]) >>
+          qexists_tac ‘NPar N2Aa N3b’ >>
+          metis_tac[trans_rules])
+      (* (FIRST DIFF) Internal Comms (TO LEFT) / Internal Comms (TO RIGHT) *)
+      >- (rename [‘trans conf (NPar N2Aa N2Ab) LTau _ ∧
+                   trans conf (NPar N2Ba N2Bb) LTau _’,
+                  ‘net_wf (NPar N1a N1b)’,
+                  ‘trans conf N1a (LReceive spA dA rpA) N2Aa’,
+                  ‘trans conf N1a (LSend spB dB rpB) N2Ba’] >>
+          ‘∃N3a.
+            trans conf N2Aa (LSend spB dB rpB) N3a ∧
+            trans conf N2Ba (LReceive spA dA rpA) N3a’
+            by (irule trans_diff_diamond >>
+                rw[compat_labels_def] >>
+                qexists_tac ‘N1a’ >>
+                fs[net_wf_def,wf_label_def,compat_labels_def] >>
+                ‘net_has_node N1b spA ∧ net_has_node N1b rpB’
+                  suffices_by metis_tac[DISJOINT_SYM,
+                                        DISJOINT_ALT,
+                                        IN_APP] >>
+                metis_tac[trans_send_cond,trans_receive_cond]) >>
+          ‘∃N3b.
+            trans conf N2Ab (LReceive spB dB rpB) N3b ∧
+            trans conf N2Bb (LSend spA dA rpA) N3b’
+            by (irule trans_diff_diamond >>
+                rw[compat_labels_def] >>
+                qexists_tac ‘N1b’ >>
+                fs[net_wf_def,wf_label_def] >>
+                ‘net_has_node N1a rpA ∧ net_has_node N1a spB’
+                  suffices_by metis_tac[DISJOINT_SYM,
+                                        DISJOINT_ALT,
+                                        IN_APP] >>
+                metis_tac[trans_send_cond,trans_receive_cond]) >>
+          qexists_tac ‘NPar N3a N3b’ >>
+          metis_tac[trans_rules])
+      (* (SECOND DIFF) Internal Comms (TO LEFT) / Internal Comms (TO RIGHT) *)
+      >- (rename [‘trans conf (NPar N2Aa N2Ab) LTau _ ∧
+                   trans conf (NPar N2Ba N2Bb) LTau _’,
+                  ‘net_wf (NPar N1a N1b)’,
+                  ‘trans conf N1a (LReceive spA dA rpA) N2Aa’,
+                  ‘trans conf N1a (LSend spB dB rpB) N2Ba’] >>
+          ‘∃N3a.
+            trans conf N2Aa (LSend spB dB rpB) N3a ∧
+            trans conf N2Ba (LReceive spA dA rpA) N3a’
+            by (irule trans_diff_diamond >>
+                rw[compat_labels_def] >>
+                qexists_tac ‘N1a’ >>
+                fs[net_wf_def,wf_label_def,compat_labels_def] >>
+                ‘net_has_node N1b spA ∧ net_has_node N1b rpB’
+                  suffices_by metis_tac[DISJOINT_SYM,
+                                        DISJOINT_ALT,
+                                        IN_APP] >>
+                metis_tac[trans_send_cond,trans_receive_cond]) >>
+          ‘∃N3b.
+            trans conf N2Ab (LReceive spB dB rpB) N3b ∧
+            trans conf N2Bb (LSend spA dA rpA) N3b’
+            by (irule trans_diff_diamond >>
+                rw[compat_labels_def] >>
+                qexists_tac ‘N1b’ >>
+                fs[net_wf_def,wf_label_def] >>
+                ‘net_has_node N1a rpA ∧ net_has_node N1a spB’
+                  suffices_by metis_tac[DISJOINT_SYM,
+                                        DISJOINT_ALT,
+                                        IN_APP] >>
+                metis_tac[trans_send_cond,trans_receive_cond]) >>
+          qexists_tac ‘NPar N3a N3b’ >>
+          metis_tac[trans_rules])
+      (* (FIRST DIFF) Internal Comms (TO LEFT) / Internal Comms (TO LEFT) *)
+      >- (rename [‘trans conf (NPar N2Aa N2Ab) LTau _ ∧
+                   trans conf (NPar N2Ba N2Bb) LTau _’,
+                  ‘net_wf (NPar N1a N1b)’,
+                  ‘trans conf N1a (LReceive spA dA rpA) N2Aa’,
+                  ‘trans conf N1a (LReceive spB dB rpB) N2Ba’] >>
+          ‘∃N3a.
+            trans conf N2Aa (LReceive spB dB rpB) N3a ∧
+            trans conf N2Ba (LReceive spA dA rpA) N3a’
+            by (irule trans_diff_diamond >>
+                rw[]
+                >- (CCONTR_TAC >>
+                    ‘N2Aa = N2Ba’
+                      suffices_by rw[] >>
+                    irule trans_notau_functional >>
+                    MAP_EVERY qexists_tac [‘LReceive spB dB rpB’,
+                                            ‘N1a’,‘conf’] >>
+                    fs[net_wf_def])
+                >- metis_tac[send_gen_compat,net_wf_def]
+                >- (qexists_tac ‘N1a’ >>
+                    fs[net_wf_def,wf_label_def] >>
+                    ‘net_has_node N1b spA ∧ net_has_node N1b spB’
+                      suffices_by metis_tac[DISJOINT_SYM,
+                                            DISJOINT_ALT,
+                                            IN_APP] >>
+                    metis_tac[trans_send_cond])) >>
+          ‘∃N3b.
+            trans conf N2Ab (LSend spB dB rpB) N3b ∧
+            trans conf N2Bb (LSend spA dA rpA) N3b’
+            by (irule trans_diff_diamond >>
+                rw[compat_labels_def]
+                >- (CCONTR_TAC >>
+                    ‘N2Aa = N2Ba’
+                      suffices_by rw[] >>
+                    irule trans_notau_functional >>
+                    MAP_EVERY qexists_tac [‘LReceive spB dB rpB’,
+                                            ‘N1a’,‘conf’] >>
+                    fs[net_wf_def])
+                >- (qexists_tac ‘N1b’ >>
+                    fs[net_wf_def,wf_label_def,compat_labels_def] >>
+                    ‘net_has_node N1a rpA ∧ net_has_node N1a rpB’
+                      suffices_by metis_tac[DISJOINT_SYM,
+                                            DISJOINT_ALT,
+                                            IN_APP] >>
+                    metis_tac[trans_receive_cond])) >>
+          qexists_tac ‘NPar N3a N3b’ >>
+          metis_tac[trans_rules])
+      (* (SECOND DIFF) Internal Comms (TO LEFT) / Internal Comms (TO LEFT) *)
+      >- (rename [‘trans conf (NPar N2Aa N2Ab) LTau _ ∧
+                   trans conf (NPar N2Ba N2Bb) LTau _’,
+                  ‘net_wf (NPar N1a N1b)’,
+                  ‘trans conf N1a (LReceive spA dA rpA) N2Aa’,
+                  ‘trans conf N1a (LReceive spB dB rpB) N2Ba’] >>
+          ‘∃N3a.
+            trans conf N2Aa (LReceive spB dB rpB) N3a ∧
+            trans conf N2Ba (LReceive spA dA rpA) N3a’
+            by (irule trans_diff_diamond >>
+                rw[]
+                >- (CCONTR_TAC >>
+                    ‘N2Ab = N2Bb’
+                      suffices_by rw[] >>
+                    irule trans_notau_functional >>
+                    MAP_EVERY qexists_tac [‘LSend spB dB rpB’,
+                                            ‘N1b’,‘conf’] >>
+                    fs[net_wf_def])
+                >- metis_tac[send_gen_compat,net_wf_def]
+                >- (qexists_tac ‘N1a’ >>
+                    fs[net_wf_def,wf_label_def] >>
+                    ‘net_has_node N1b spA ∧ net_has_node N1b spB’
+                      suffices_by metis_tac[DISJOINT_SYM,
+                                            DISJOINT_ALT,
+                                            IN_APP] >>
+                    metis_tac[trans_send_cond])) >>
+          ‘∃N3b.
+            trans conf N2Ab (LSend spB dB rpB) N3b ∧
+            trans conf N2Bb (LSend spA dA rpA) N3b’
+            by (irule trans_diff_diamond >>
+                rw[compat_labels_def]
+                >- (CCONTR_TAC >>
+                    ‘N2Ab = N2Bb’
+                      suffices_by rw[] >>
+                    irule trans_notau_functional >>
+                    MAP_EVERY qexists_tac [‘LSend spB dB rpB’,
+                                            ‘N1b’,‘conf’] >>
+                    fs[net_wf_def])
+                >- (qexists_tac ‘N1b’ >>
+                    fs[net_wf_def,wf_label_def,compat_labels_def] >>
+                    ‘net_has_node N1a rpA ∧ net_has_node N1a rpB’
+                      suffices_by metis_tac[DISJOINT_SYM,
+                                            DISJOINT_ALT,
+                                            IN_APP] >>
+                    metis_tac[trans_receive_cond])) >>
+          qexists_tac ‘NPar N3a N3b’ >>
+          metis_tac[trans_rules])
+      (* (FIRST DIFF) Internal Comms (TO LEFT) / Parallel Embedded Behaviour (LEFT) *)
+      >- (rename [‘trans conf (NPar N2Aa N2Ab) LTau _ ∧
+                   trans conf (NPar N2Ba N1b) LTau _’,
+                  ‘net_wf (NPar N1a N1b)’,
+                  ‘trans conf N1a (LReceive sp d rp) N2Aa’] >>
+          ‘∃N3a.
+            trans conf N2Aa LTau N3a ∧
+            trans conf N2Ba (LReceive sp d rp) N3a’
+            by (irule trans_diff_diamond >>
+                rw[compat_labels_def] >>
+                qexists_tac ‘N1a’ >>
+                fs[net_wf_def,wf_label_def,compat_labels_def] >>
+                ‘net_has_node N1b sp’
+                      suffices_by metis_tac[DISJOINT_SYM,
+                                            DISJOINT_ALT,
+                                            IN_APP] >>
+                metis_tac[trans_send_cond]) >>
+          qexists_tac ‘NPar N3a N2Ab’ >>
+          metis_tac[trans_rules])
+      (* (SECOND DIFF) Internal Comms (TO LEFT) / Parallel Embedded Behaviour (LEFT) *)
+      >- (rename [‘trans conf (NPar N2Aa N2Ab) LTau _ ∧
+                   trans conf (NPar N2Ba N1b) LTau _’,
+                  ‘net_wf (NPar N1a N1b)’,
+                  ‘trans conf N1a (LReceive sp d rp) N2Aa’] >>
+          ‘∃N3a.
+            trans conf N2Aa LTau N3a ∧
+            trans conf N2Ba (LReceive sp d rp) N3a’
+            by (irule trans_diff_diamond >>
+                rw[compat_labels_def] >>
+                qexists_tac ‘N1a’ >>
+                fs[net_wf_def,wf_label_def,compat_labels_def] >>
+                ‘net_has_node N1b sp’
+                      suffices_by metis_tac[DISJOINT_SYM,
+                                            DISJOINT_ALT,
+                                            IN_APP] >>
+                metis_tac[trans_send_cond]) >>
+          qexists_tac ‘NPar N3a N2Ab’ >>
+          metis_tac[trans_rules])
+      (* (FIRST DIFF) Internal Comms (TO LEFT) / Parallel Embedded Behaviour (RIGHT) *)
+      >- (rename [‘trans conf (NPar N2Aa N2Ab) LTau _ ∧
+                   trans conf (NPar N1a N2Bb) LTau _’,
+                  ‘net_wf (NPar N1a N1b)’,
+                  ‘trans conf N1a (LReceive sp d rp) N2Aa’] >>
+          ‘∃N3b.
+            trans conf N2Ab LTau N3b ∧
+            trans conf N2Bb (LSend sp d rp) N3b’
+            by (irule trans_diff_diamond >>
+                rw[compat_labels_def] >>
+                qexists_tac ‘N1b’ >>
+                fs[net_wf_def,wf_label_def,compat_labels_def] >>
+                ‘net_has_node N1a rp’
+                      suffices_by metis_tac[DISJOINT_SYM,
+                                            DISJOINT_ALT,
+                                            IN_APP] >>
+                metis_tac[trans_receive_cond]) >>
+          qexists_tac ‘NPar N2Aa N3b’ >>
+          metis_tac[trans_rules])
+      (* (SECOND DIFF) Internal Comms (TO LEFT) / Parallel Embedded Behaviour (RIGHT) *)
+      >- (rename [‘trans conf (NPar N2Aa N2Ab) LTau _ ∧
+                   trans conf (NPar N1a N2Bb) LTau _’,
+                  ‘net_wf (NPar N1a N1b)’,
+                  ‘trans conf N1a (LReceive sp d rp) N2Aa’] >>
+          ‘∃N3b.
+            trans conf N2Ab LTau N3b ∧
+            trans conf N2Bb (LSend sp d rp) N3b’
+            by (irule trans_diff_diamond >>
+                rw[compat_labels_def] >>
+                qexists_tac ‘N1b’ >>
+                fs[net_wf_def,wf_label_def,compat_labels_def] >>
+                ‘net_has_node N1a rp’
+                      suffices_by metis_tac[DISJOINT_SYM,
+                                            DISJOINT_ALT,
+                                            IN_APP] >>
+                metis_tac[trans_receive_cond]) >>
+          qexists_tac ‘NPar N2Aa N3b’ >>
+          metis_tac[trans_rules])
+      (* (FIRST DIFF) Parallel Embedded Behaviour (LEFT) / Internal Comms (TO RIGHT) *)
+      >- (rename [‘trans conf (NPar N2Ba N1b) LTau _ ∧
+                   trans conf (NPar N2Aa N2Ab) LTau _’,
+                  ‘net_wf (NPar N1a N1b)’,
+                  ‘trans conf N1a (LSend sp d rp) N2Aa’] >>
+          ‘∃N3a.
+            trans conf N2Aa LTau N3a ∧
+            trans conf N2Ba (LSend sp d rp) N3a’
+            by (irule trans_diff_diamond >>
+                rw[compat_labels_def] >>
+                qexists_tac ‘N1a’ >>
+                fs[net_wf_def,wf_label_def,compat_labels_def] >>
+                ‘net_has_node N1b rp’
+                      suffices_by metis_tac[DISJOINT_SYM,
+                                            DISJOINT_ALT,
+                                            IN_APP] >>
+                metis_tac[trans_receive_cond]) >>
+          qexists_tac ‘NPar N3a N2Ab’ >>
+          metis_tac[trans_rules])
+      (* (SECOND DIFF) Parallel Embedded Behaviour (LEFT) / Internal Comms (TO RIGHT) *)
+      >- (rename [‘trans conf (NPar N2Ba N1b) LTau _ ∧
+                   trans conf (NPar N2Aa N2Ab) LTau _’,
+                  ‘net_wf (NPar N1a N1b)’,
+                  ‘trans conf N1a (LSend sp d rp) N2Aa’] >>
+          ‘∃N3a.
+            trans conf N2Aa LTau N3a ∧
+            trans conf N2Ba (LSend sp d rp) N3a’
+            by (irule trans_diff_diamond >>
+                rw[compat_labels_def] >>
+                qexists_tac ‘N1a’ >>
+                fs[net_wf_def,wf_label_def,compat_labels_def] >>
+                ‘net_has_node N1b rp’
+                      suffices_by metis_tac[DISJOINT_SYM,
+                                            DISJOINT_ALT,
+                                            IN_APP] >>
+                metis_tac[trans_receive_cond]) >>
+          qexists_tac ‘NPar N3a N2Ab’ >>
+          metis_tac[trans_rules])
+      (* (FIRST DIFF) Parallel Embedded Behaviour (LEFT) / Internal Comms (TO LEFT) *)
+      >- (rename [‘trans conf (NPar N2Ba N1b) LTau _ ∧
+                   trans conf (NPar N2Aa N2Ab) LTau _’,
+                  ‘net_wf (NPar N1a N1b)’,
+                  ‘trans conf N1a (LReceive sp d rp) N2Aa’] >>
+          ‘∃N3a.
+            trans conf N2Aa LTau N3a ∧
+            trans conf N2Ba (LReceive sp d rp) N3a’
+            by (irule trans_diff_diamond >>
+                rw[compat_labels_def] >>
+                qexists_tac ‘N1a’ >>
+                fs[net_wf_def,wf_label_def,compat_labels_def] >>
+                ‘net_has_node N1b sp’
+                      suffices_by metis_tac[DISJOINT_SYM,
+                                            DISJOINT_ALT,
+                                            IN_APP] >>
+                metis_tac[trans_send_cond]) >>
+          qexists_tac ‘NPar N3a N2Ab’ >>
+          metis_tac[trans_rules])
+      (* (SECOND DIFF) Parallel Embedded Behaviour (LEFT) / Internal Comms (TO LEFT) *)
+      >- (rename [‘trans conf (NPar N2Ba N1b) LTau _ ∧
+                   trans conf (NPar N2Aa N2Ab) LTau _’,
+                  ‘net_wf (NPar N1a N1b)’,
+                  ‘trans conf N1a (LReceive sp d rp) N2Aa’] >>
+          ‘∃N3a.
+            trans conf N2Aa LTau N3a ∧
+            trans conf N2Ba (LReceive sp d rp) N3a’
+            by (irule trans_diff_diamond >>
+                rw[compat_labels_def] >>
+                qexists_tac ‘N1a’ >>
+                fs[net_wf_def,wf_label_def,compat_labels_def] >>
+                ‘net_has_node N1b sp’
+                      suffices_by metis_tac[DISJOINT_SYM,
+                                            DISJOINT_ALT,
+                                            IN_APP] >>
+                metis_tac[trans_send_cond]) >>
+          qexists_tac ‘NPar N3a N2Ab’ >>
+          metis_tac[trans_rules])
+      (* (FIRST DIFF) Parallel Embedded Behaviour (LEFT) / Parallel Embedded Behaviour (LEFT) *)
+      >- (rename [‘trans conf (NPar N2Aa N1b) LTau _ ∧
+                   trans conf (NPar N2Ba N1b) LTau _’,
+                  ‘net_wf (NPar N1a N1b)’] >>
+          ‘∃N3a.
+            trans conf N2Aa LTau N3a ∧
+            trans conf N2Ba LTau N3a’
+            by metis_tac[net_wf_def] >>
+          qexists_tac ‘NPar N3a N1b’ >>
+          metis_tac[trans_rules])
+      (* Note: SECOND DIFF of dual parallel embedded left behaviour not possible! *)
+      (* (FIRST DIFF) Parallel Embedded Behaviour (LEFT) / Parallel Embedded Behaviour (RIGHT) *)
+      >- (rename [‘trans conf (NPar N2Aa N1b) LTau _ ∧
+                   trans conf (NPar N1a N2Bb) LTau _’,
+                  ‘net_wf (NPar N1a N1b)’] >>
+          metis_tac[trans_rules])
+      (* (SECOND DIFF) Parallel Embedded Behaviour (LEFT) / Parallel Embedded Behaviour (RIGHT) *)
+      >- (rename [‘trans conf (NPar N2Aa N1b) LTau _ ∧
+                   trans conf (NPar N1a N2Bb) LTau _’,
+                  ‘net_wf (NPar N1a N1b)’] >>
+          metis_tac[trans_rules])
+      (* (FIRST DIFF) Parallel Embedded Behaviour (RIGHT) / Internal Comms (TO RIGHT) *)
+      >- (rename [‘trans conf (NPar N1a N2Bb) LTau _ ∧
+                   trans conf (NPar N2Aa N2Ab) LTau _’,
+                  ‘net_wf (NPar N1a N1b)’,
+                  ‘trans conf N1a (LSend sp d rp) N2Aa’] >>
+          ‘∃N3b.
+            trans conf N2Ab LTau N3b ∧
+            trans conf N2Bb (LReceive sp d rp) N3b’
+            by (irule trans_diff_diamond >>
+                rw[compat_labels_def] >>
+                qexists_tac ‘N1b’ >>
+                fs[net_wf_def,wf_label_def,compat_labels_def] >>
+                ‘net_has_node N1a sp’
+                      suffices_by metis_tac[DISJOINT_SYM,
+                                            DISJOINT_ALT,
+                                            IN_APP] >>
+                metis_tac[trans_send_cond]) >>
+          qexists_tac ‘NPar N2Aa N3b’ >>
+          metis_tac[trans_rules])
+      (* (SECOND DIFF) Parallel Embedded Behaviour (RIGHT) / Internal Comms (TO RIGHT) *)
+      >- (rename [‘trans conf (NPar N1a N2Bb) LTau _ ∧
+                   trans conf (NPar N2Aa N2Ab) LTau _ ’,
+                  ‘net_wf (NPar N1a N1b)’,
+                  ‘trans conf N1a (LSend sp d rp) N2Aa’] >>
+          ‘∃N3b.
+            trans conf N2Ab LTau N3b ∧
+            trans conf N2Bb (LReceive sp d rp) N3b’
+            by (irule trans_diff_diamond >>
+                rw[compat_labels_def] >>
+                qexists_tac ‘N1b’ >>
+                fs[net_wf_def,wf_label_def,compat_labels_def] >>
+                ‘net_has_node N1a sp’
+                      suffices_by metis_tac[DISJOINT_SYM,
+                                            DISJOINT_ALT,
+                                            IN_APP] >>
+                metis_tac[trans_send_cond]) >>
+          qexists_tac ‘NPar N2Aa N3b’ >>
+          metis_tac[trans_rules])
+      (* (FIRST DIFF) Parallel Embedded Behaviour (RIGHT) / Internal Comms (TO LEFT) *)
+      >- (rename [‘trans conf (NPar N1a N2Bb) LTau _ ∧
+                   trans conf (NPar N2Aa N2Ab) LTau _ ’,
+                  ‘net_wf (NPar N1a N1b)’,
+                  ‘trans conf N1a (LReceive sp d rp) N2Aa’] >>
+          ‘∃N3b.
+            trans conf N2Ab LTau N3b ∧
+            trans conf N2Bb (LSend sp d rp) N3b’
+            by (irule trans_diff_diamond >>
+                rw[compat_labels_def] >>
+                qexists_tac ‘N1b’ >>
+                fs[net_wf_def,wf_label_def,compat_labels_def] >>
+                ‘net_has_node N1a rp’
+                      suffices_by metis_tac[DISJOINT_SYM,
+                                            DISJOINT_ALT,
+                                            IN_APP] >>
+                metis_tac[trans_receive_cond]) >>
+          qexists_tac ‘NPar N2Aa N3b’ >>
+          metis_tac[trans_rules])
+      (* (SECOND DIFF) Parallel Embedded Behaviour (RIGHT) / Internal Comms (TO LEFT) *)
+      >- (rename [‘trans conf (NPar N1a N2Bb) LTau _ ∧
+                   trans conf (NPar N2Aa N2Ab) LTau _ ’,
+                  ‘net_wf (NPar N1a N1b)’,
+                  ‘trans conf N1a (LReceive sp d rp) N2Aa’] >>
+          ‘∃N3b.
+            trans conf N2Ab LTau N3b ∧
+            trans conf N2Bb (LSend sp d rp) N3b’
+            by (irule trans_diff_diamond >>
+                rw[compat_labels_def] >>
+                qexists_tac ‘N1b’ >>
+                fs[net_wf_def,wf_label_def,compat_labels_def] >>
+                ‘net_has_node N1a rp’
+                      suffices_by metis_tac[DISJOINT_SYM,
+                                            DISJOINT_ALT,
+                                            IN_APP] >>
+                metis_tac[trans_receive_cond]) >>
+          qexists_tac ‘NPar N2Aa N3b’ >>
+          metis_tac[trans_rules])
+      (* (FIRST DIFF) Parallel Embedded Behaviour (RIGHT) / Parallel Embedded Behaviour (LEFT) *)
+      >- (rename [‘trans conf (NPar N1a N2Bb) LTau _ ∧
+                   trans conf (NPar N2Aa N1b) LTau _’,
+                  ‘net_wf (NPar N1a N1b)’] >>
+          metis_tac[trans_rules])
+      (* (SECOND DIFF) Parallel Embedded Behaviour (LEFT) / Parallel Embedded Behaviour (RIGHT) *)
+      >- (rename [‘trans conf (NPar N1a N2Bb) LTau _ ∧
+                   trans conf (NPar N2Aa N1b) LTau _’,
+                  ‘net_wf (NPar N1a N1b)’] >>
+          metis_tac[trans_rules])
+      (* (FIRST DIFF) Parallel Embedded Behaviour (RIGHT) / Parallel Embedded Behaviour (RIGHT) *)
+      >- (rename [‘trans conf (NPar N1a N2Ab) LTau _ ∧
+                   trans conf (NPar N1a N2Bb) LTau _’,
+                  ‘net_wf (NPar N1a N1b)’] >>
+          ‘∃N3b.
+            trans conf N2Ab LTau N3b ∧
+            trans conf N2Bb LTau N3b’
+            by metis_tac[net_wf_def] >>
+          qexists_tac ‘NPar N1a N3b’ >>
+          metis_tac[trans_rules])
+      (* Note: SECOND DIFF of dual parallel embedded right behaviour not possible! *)
+      )
+  (* NEndpoint case *)
+  >- (rw[] >>
+      qpat_x_assum ‘trans _ _ _ N2A’
+                  (fn x => strip_assume_tac(REWRITE_RULE [Once trans_cases] x)) >>
+      fs[] >> rw[] >> fs[] >>
+      qpat_x_assum ‘trans _ _ _ N2B’
+                  (fn x => strip_assume_tac(REWRITE_RULE [Once trans_cases] x)) >>
+      fs[] >> rw[] >> fs[] >>
+      metis_tac[final_inter_mutexc])
+QED
+
+(*  General Reflexive Confluence Result*)
+Theorem trans_diamond:
+  ∀conf N1 LA N2A LB N2B.
+    net_wf N1 ∧
+    wf_label N1 LA ∧
+    wf_label N1 LB ∧
+    compat_labels LA LB ∧
+    trans conf N1 LA N2A ∧
+    trans conf N1 LB N2B ⇒
+    ∃N3.
+      RC (λn1 n2. trans conf n1 LB n2) N2A N3 ∧
+      RC (λn1 n2. trans conf n1 LA n2) N2B N3
+Proof
+  rw[] >>
+  Cases_on ‘LA = LB’
+  >- (Cases_on ‘LA = LTau’ >> rw[RC_DEF]
+      >- (rw[RC_DEF] >>
+          metis_tac[trans_samelab_tau_difout_diamond])
+      >- metis_tac[RC_DEF,trans_notau_functional])
+  >- (rw[RC_DEF] >> metis_tac[trans_diff_diamond])
 QED
 
 val _ = export_theory ();
