projection/proofs/to_cake/ffi/comms_ffi_eqScript.sml
@@ -1,0 +1,666 @@
+open HolKernel boolLib Parse bossLib;
+open optionTheory
+     relationTheory;
+open ffiTheory;
+open bisimulationTheory
+     bisimulation_extTheory
+     confluenceTheory
+     payloadPropsTheory
+     payloadSemTheory
+     payloadLangTheory
+     comms_ffi_modelTheory
+     comms_ffi_propsTheory
+     comms_ffi_consTheory
+     comms_ffi_commTheory;
+
+val _ = new_theory "comms_ffi_eq";
+
+(* FFI STATE EQUIVALENCE *)
+(* Definition *)
+Definition ffi_eq_def:
+  ffi_eq conf = BISIM_REL (strans conf)
+End
+
+(* Basic equivalence property *)
+Theorem ffi_eq_equivRel:
+  ∀conf. equivalence (ffi_eq conf)
+Proof
+  rw [ffi_eq_def,BISIM_REL_IS_EQUIV_REL]
+QED
+
+(* Irrelevance if queues are similar *)
+Theorem qsame_irrel_ffi_eq:
+  ∀c q1 q2 N.
+    qsame q1 q2 ⇒
+    ffi_eq conf (c,q1,N) (c,q2,N)
+Proof
+  simp[ffi_eq_def,bi_is_BISIM_REL] >>
+  ‘∀s1 s2.
+    (λ(c1,q1,N1) (c2,q2,N2).
+      c1 = c2 ∧
+      N1 = N2 ∧
+     qsame q1 q2) s1 s2 ⇒
+    bi (strans conf) s1 s2’
+    suffices_by (rw[] >> metis_tac[pairTheory.FORALL_PROD]) >>
+  ho_match_mp_tac bi_coind >> rw[] >>
+  rename1 ‘strans conf _ L sO’ >>
+  MAP_EVERY PairCases_on [‘s1’,‘s2’,‘sO’] >>
+  fs[] >> rw[] >>
+  last_x_assum mp_tac >>
+  pop_assum mp_tac >> rw[] >> Cases_on ‘L’ >>
+  ‘sO0 = s10’
+    by metis_tac[pairTheory.FST,strans_pres_pnum] >>
+  fs[strans_send_equiv,strans_receive_equiv,pairTheory.EXISTS_PROD]
+  >- (MAP_EVERY (drule_all_then strip_assume_tac)
+                [qsame_irrel_active,
+                 qsame_irrel_send,
+                 qsame_irrel_internal] >>
+      rename1 ‘input_trans conf _ (q2MA,_) _ (q2MB,_)’ >>
+      ‘q2MA = q2MB’
+        by fs[input_trans_def] >>
+      rw[] >> metis_tac[])
+  >- (MAP_EVERY (drule_all_then strip_assume_tac)
+                [qsame_irrel_active,
+                 qsame_irrel_receive] >>
+      fs[] >>
+      drule_all_then strip_assume_tac qsame_irrel_internal >>
+      rw[] >> metis_tac[])
+  >- (‘∀(x : word8 list |-> word8 list list) y. qsame x y ⇔ qsame y x’
+        by (rw[qsame_def] >> metis_tac[]) >>
+      rename1 ‘qsame A B’ >>
+      ‘qsame B A’ by metis_tac[] >>
+      MAP_EVERY (drule_all_then strip_assume_tac)
+                [qsame_irrel_active,
+                 qsame_irrel_send,
+                 qsame_irrel_internal] >>
+      rename1 ‘input_trans conf _ (q2MA,_) _ (q2MB,_)’ >>
+      ‘q2MA = q2MB’
+        by fs[input_trans_def] >>
+      rw[] >> metis_tac[])
+  >- (‘∀(x : word8 list |-> word8 list list) y. qsame x y ⇔ qsame y x’
+        by (rw[qsame_def] >> metis_tac[]) >>
+      rename1 ‘qsame A B’ >>
+      ‘qsame B A’ by metis_tac[] >>
+      MAP_EVERY (drule_all_then strip_assume_tac)
+                [qsame_irrel_active,
+                 qsame_irrel_receive] >>
+      fs[] >>
+      drule_all_then strip_assume_tac qsame_irrel_internal >>
+      rw[] >> metis_tac[])
+QED
+
+(* DECONSTRUCTION PIECES EQUIVALENCE PRESERVATION *)
+(* General Theorems *)
+(* -- Equiv. irrel. gives equiv. pres. *)
+Theorem equiv_irrel_pres:
+  ∀ts.
+    (* ASSUMPTIONS *)
+    (* 1. RTC ts is irrelevant to equivalence *)
+    (∀conf c q1 N1 q2 N2.
+      ffi_wf (c,q1,N1) ∧
+      RTC (ts conf c) (q1,N1) (q2,N2) ⇒
+      ffi_eq conf (c,q1,N1) (c,q2,N2)) ⇒
+    (* CONCLUSION *)
+    (* RTC ts preserves equivalence *)
+    (∀conf cA q1A N1A q2A N2A cB q1B N1B q2B N2B.
+      ffi_wf (cA,q1A,N1A) ∧
+      ffi_wf (cB,q1B,N1B) ∧
+      ffi_eq conf (cA,q1A,N1A) (cB,q1B,N1B) ∧
+      RTC (ts conf cA) (q1A,N1A) (q2A,N2A)       ∧
+      RTC (ts conf cB) (q1B,N1B) (q2B,N2B)       ⇒
+      ffi_eq conf (cA,q2A,N2A) (cB,q2B,N2B))
+Proof
+  rw[] >>
+  metis_tac[ffi_eq_equivRel,equivalence_def,
+                          transitive_def,symmetric_def]
+QED
+
+(* -- strans comm. + subset of active_trans gives equiv. pres. *)
+Theorem equiv_irrel_cond:
+  ∀ts.
+    (* ASSUMPTIONS *)
+    (* 1. ts is a subset of active_trans *)
+    (∀conf c q1 N1 q2 N2.
+      ts conf c (q1,N1) (q2,N2) ⇒
+      active_trans conf c (q1,N1) (q2,N2)) ∧
+    (* 2. RTC ts commutes with strans *)
+    (∀conf c q1 N1 L q2S N2S q2T N2T.
+      ffi_wf (c,q1,N1) ∧
+      strans conf (c,q1,N1) L (c,q2S,N2S) ∧
+      RTC (ts conf c) (q1,N1) (q2T,N2T) ⇒
+      ∃q3 N3.
+        RTC (ts conf c) (q2S,N2S) (q3,N3) ∧
+        strans conf (c,q2T,N2T) L (c,q3,N3)) ⇒
+    (* CONCLUSION *)
+    (* RTC ts is irrelevant to equivalence *)
+    (∀conf c q1 N1 q2 N2.
+      ffi_wf (c,q1,N1) ∧
+      RTC (ts conf c) (q1,N1) (q2,N2) ⇒
+      ffi_eq conf (c,q1,N1) (c,q2,N2))
+Proof
+  ntac 3 strip_tac >>
+  simp[ffi_eq_def,bi_is_BISIM_REL] >>
+  gen_tac >>
+  ‘∀s1 s2.
+    (λ (c1,q1,N1) (c2,q2,N2).
+      c1 = c ∧
+      c2 = c ∧
+      ffi_wf (c,q1,N1) ∧
+      RTC (ts conf c) (q1,N1) (q2,N2)) s1 s2
+    ⇒ bi (strans conf) s1 s2’
+    suffices_by rw[] >>
+  ho_match_mp_tac bi_coind >>
+  rw[] >>
+  PairCases_on ‘s1’ >> PairCases_on ‘s2’ >>
+  fs[] >> rfs[]
+  >- (rename [‘strans conf _ L s3’,
+              ‘∃x. strans conf _ L x ∧
+                   _ s3 x’] >>
+      ‘FST s3 = c’
+        by metis_tac[strans_pres_pnum,
+                     pairTheory.FST] >>
+      PairCases_on ‘s3’ >>
+      fs[] >>
+      pop_assum (K ALL_TAC) >>
+      pop_assum mp_tac >>
+      qpat_x_assum ‘ffi_wf (c,s11,s12)’ mp_tac >>
+      pop_assum mp_tac >>
+      qabbrev_tac ‘s1 = (s11,s12)’ >>
+      qabbrev_tac ‘s2a = (s21,s22)’ >>
+      qabbrev_tac ‘s2b = (s31,s32)’ >>
+      ntac 5 (pop_assum (K ALL_TAC)) >>
+      MAP_EVERY qid_spec_tac [‘s2b’,‘s2a’,‘s1’] >>
+      Induct_on ‘RTC’ >> rw[]
+      >- (qexists_tac ‘(c,s2b)’ >> rw[] >>
+          PairCases_on ‘s2b’ >> rw[] >>
+          metis_tac[strans_pres_wf])
+      >- (rename1 ‘ts conf c s1 si’ >>
+          PairCases_on ‘s1’ >> PairCases_on ‘si’ >>
+          PairCases_on ‘s2b’ >>
+          ‘∃siM0 siM1. strans conf (c,si0,si1) L (c,siM0,siM1) ∧
+                 RTC (ts conf c) (s2b0,s2b1) (siM0,siM1)’
+            by metis_tac[RTC_SINGLE] >>
+          ‘ffi_wf (c,si0,si1)’
+            by metis_tac[active_trans_pres_wf,RTC_SINGLE] >>
+          first_x_assum (drule_all_then strip_assume_tac) >>
+          rename1 ‘strans conf (c,s2a) L s3’ >>
+          qexists_tac ‘s3’ >>
+          PairCases_on ‘s3’ >>
+          fs[] >>
+          metis_tac[strans_pres_wf,RTC_SINGLE,
+                    RTC_TRANSITIVE,transitive_def]))
+  >- (rename [‘strans conf _ L s3’,
+              ‘∃x. strans conf _ L x ∧
+                   _ x s3’] >>
+      qexists_tac ‘s3’ >>
+      ‘RTC (active_trans conf c) (s11,s12) (s21,s22)’
+        suffices_by (‘FST s3 = c’
+                        by metis_tac[strans_pres_pnum,
+                                     pairTheory.FST] >>
+                     PairCases_on ‘s3’ >>
+                     fs[] >>
+                     metis_tac[strans_pres_pnum,
+                               strans_front_construct,
+                               strans_pres_wf]) >>
+      pop_assum (K ALL_TAC) >>
+      qpat_x_assum ‘ffi_wf (c,s11,s12)’ mp_tac >>
+      pop_assum mp_tac >>
+      qabbrev_tac ‘sa = (s11,s12)’ >>
+      qabbrev_tac ‘sb = (s21,s22)’ >>
+      ntac 5 (pop_assum (K ALL_TAC)) >>
+      MAP_EVERY qid_spec_tac [‘sb’,‘sa’] >>
+      Induct_on ‘RTC’ >> rw[] >>
+      rename1 ‘ts conf c sa si’ >>
+      ‘active_trans conf c sa si’
+        suffices_by (‘ffi_wf (c,si)’
+                      by (MAP_EVERY PairCases_on [‘sa’,‘si’] >>
+                          metis_tac[active_trans_pres_wf,RTC_SINGLE]) >>
+                    metis_tac[RTC_SINGLE,RTC_TRANSITIVE,transitive_def]) >>
+      PairCases_on ‘sa’ >> PairCases_on ‘si’ >> metis_tac[])
+QED
+
+(* Equivalence Preservation for Specific Pieces *)
+(* -- Internal *)
+(* -- -- Equivalence Irrelevance *)
+Theorem internal_trans_equiv_irrel:
+  ∀conf c q1 N1 q2 N2.
+    ffi_wf (c,q1,N1) ∧
+    RTC (internal_trans conf c) (q1,N1) (q2,N2) ⇒
+    ffi_eq conf (c,q1,N1) (c,q2,N2)
+Proof
+  rw[] >>
+  metis_tac[equiv_irrel_cond,active_trans_def,
+            internal_strans_comm]
+QED
+
+(* -- -- Equivalence Preservation *)
+Theorem internal_trans_equiv_pres:
+  ∀conf cA q1A N1A q2A N2A cB q1B N1B q2B N2B.
+    ffi_wf (cA,q1A,N1A) ∧
+    ffi_wf (cB,q1B,N1B) ∧
+    ffi_eq conf (cA,q1A,N1A) (cB,q1B,N1B)       ∧
+    RTC (internal_trans conf cA) (q1A,N1A) (q2A,N2A) ∧
+    RTC (internal_trans conf cB) (q1B,N1B) (q2B,N2B)   ⇒
+      ffi_eq conf (cA,q2A,N2A) (cB,q2B,N2B)
+Proof
+  rw[] >>
+  irule equiv_irrel_pres >>
+  metis_tac[internal_trans_equiv_irrel]
+QED
+
+(* -- Active Bisim preservation *)
+Theorem active_trans_equiv_irrel:
+  ∀conf c q1 N1 q2 N2.
+    ffi_wf (c,q1,N1) ∧
+    RTC (active_trans conf c) (q1,N1) (q2,N2) ⇒
+    ffi_eq conf (c,q1,N1) (c,q2,N2)
+Proof
+  rw[] >>
+  metis_tac[equiv_irrel_cond,
+            active_strans_comm]
+QED
+
+Theorem active_trans_equiv_pres:
+  ∀conf cA q1A N1A q2A N2A cB q1B N1B q2B N2B.
+    ffi_wf (cA,q1A,N1A) ∧
+    ffi_wf (cB,q1B,N1B) ∧
+    ffi_eq conf (cA,q1A,N1A) (cB,q1B,N1B)       ∧
+    RTC (active_trans conf cA) (q1A,N1A) (q2A,N2A) ∧
+    RTC (active_trans conf cB) (q1B,N1B) (q2B,N2B)   ⇒
+      ffi_eq conf (cA,q2A,N2A) (cB,q2B,N2B)
+Proof
+  rw[] >>
+  irule equiv_irrel_pres >>
+  metis_tac[active_trans_equiv_irrel]
+QED
+
+
+(* FFI Receive/Network Send Transition *)
+(* -- Send Transition Bisim preservation *)
+Theorem send_trans_equiv_pres:
+  ∀conf cA q1A N1A q2A N2A rp d cB q1B N1B q2B N2B.
+    ffi_wf (cA,q1A,N1A) ∧
+    ffi_wf (cB,q1B,N1B) ∧
+    ffi_eq conf (cA,q1A,N1A) (cB,q1B,N1B)       ∧
+    input_trans conf cA (q1A,N1A) (rp,d) (q2A,N2A) ∧
+    input_trans conf cB (q1B,N1B) (rp,d) (q2B,N2B)   ⇒
+      ffi_eq conf (cA,q2A,N2A) (cB,q2B,N2B)
+Proof
+  rw[] >>
+  ‘∃q2Bb N2Bb.
+    strans conf (cB,q1B,N1B) (ASend rp d) (cB,q2Bb,N2Bb) ∧
+    ffi_eq conf (cA,q2A,N2A) (cB,q2Bb,N2Bb)’
+    by (pop_assum (K ALL_TAC) >>
+        ntac 2 (last_x_assum (K ALL_TAC)) >>
+        ‘strans conf (cA,q1A,N1A) (ASend rp d) (cA,q2A,N2A)’
+          by (irule strans_send_construct >>
+              ‘q2A = q1A’
+                by fs[input_trans_def] >>
+              fs[] >>
+              MAP_EVERY qexists_tac [‘N1A’,‘N2A’,‘q1A’] >>
+              metis_tac[RTC_REFL]) >>
+        qpat_x_assum ‘input_trans _ _ _ _ _’ (K ALL_TAC) >>
+        last_x_assum (strip_assume_tac o
+                      REWRITE_RULE [ffi_eq_def,
+                                    BISIM_REL_def,
+                                    BISIM_def]) >>
+        fs[] >>
+        rename1 ‘BR _ _’ >>
+        ‘∃c3 q3 N3.
+          strans conf (cB,q1B,N1B) (ASend rp d) (c3,q3,N3) ∧
+          BR (cA,q2A,N2A) (c3,q3,N3)’
+          by (fs[pairTheory.FORALL_PROD,
+                 pairTheory.EXISTS_PROD] >>
+              metis_tac[]) >>
+        MAP_EVERY qexists_tac [‘q3’,‘N3’] >>
+        ‘c3 = cB’
+          suffices_by (rw[ffi_eq_def,BISIM_REL_def,
+                          BISIM_def] >>
+                       metis_tac[]) >>
+        metis_tac[strans_pres_pnum,pairTheory.FST]) >>
+  fs[strans_send_equiv] >>
+  rename[‘RTC (active_trans conf cB) (q1B,N1B) (qIBa,NIBa)’,
+         ‘input_trans conf cB (qIBa,NIBa) (rp,d) (qIBb,NIBb)’,
+         ‘RTC (internal_trans conf cB) (qIBb,NIBb) (q2Bb,N2Bb)’] >>
+  ‘ffi_eq conf (cB,qIBb,NIBb) (cA,q2A,N2A)’
+    by (‘ffi_eq conf (cB,qIBb,NIBb) (cB,q2Bb,N2Bb)’
+          suffices_by metis_tac[ffi_eq_equivRel,equivalence_def,
+                                symmetric_def,transitive_def] >>
+        metis_tac[active_trans_pres_wf,
+                  input_trans_pres_wf,
+                  internal_trans_equiv_irrel]) >>
+  ‘ffi_eq conf (cB,q2B,N2B) (cB,qIBb,NIBb)’
+    suffices_by metis_tac[ffi_eq_equivRel,equivalence_def,
+                                symmetric_def,transitive_def] >>
+  drule_all_then strip_assume_tac active_send_comm >>
+  rename [‘input_trans conf cB (qIBb,NIBa) (rp,d) NS’,
+          ‘input_trans conf cB (qIBb,NIBa) (rp,d) (qOS,NOS)’] >>
+  ‘NS = (qOS,NOS)’
+    suffices_by (rw[] >>
+                 metis_tac[input_trans_pres_wf,
+                           active_trans_equiv_irrel]) >>
+  PairCases_on ‘NS’ >> fs[input_trans_def] >>
+  irule trans_notau_functional >>
+  MAP_EVERY qexists_tac [‘LReceive cB d rp’,‘NIBa’,‘conf’] >>
+  rw[] >> metis_tac[ffi_wf_def,active_trans_pres_wf]
+QED
+
+(* -- Receive Transition Bisim preservation *)
+Theorem receive_trans_equiv_pres:
+  ∀conf cA q1A N1A q2A N2A sp d cB q1B N1B q2B N2B.
+    ffi_wf (cA,q1A,N1A) ∧
+    ffi_wf (cB,q1B,N1B) ∧
+    ffi_eq conf (cA,q1A,N1A) (cB,q1B,N1B)       ∧
+    output_trans conf cA (q1A,N1A) (sp,d) (q2A,N2A) ∧
+    output_trans conf cB (q1B,N1B) (sp,d) (q2B,N2B)   ⇒
+      ffi_eq conf (cA,q2A,N2A) (cB,q2B,N2B)
+Proof
+  rw[] >>
+  ‘∃q2Bb N2Bb.
+    strans conf (cB,q1B,N1B) (ARecv sp d) (cB,q2Bb,N2Bb) ∧
+    ffi_eq conf (cA,q2A,N2A) (cB,q2Bb,N2Bb)’
+    by (pop_assum (K ALL_TAC) >>
+        ntac 2 (last_x_assum (K ALL_TAC)) >>
+        ‘strans conf (cA,q1A,N1A) (ARecv sp d) (cA,q2A,N2A)’
+          by (irule strans_receive_construct >>
+              ‘N1A = N2A’
+                by fs[output_trans_def] >>
+              fs[] >>
+              MAP_EVERY qexists_tac [‘N2A’,‘q1A’,‘q2A’] >>
+              metis_tac[RTC_REFL]) >>
+        qpat_x_assum ‘output_trans _ _ _ _ _’ (K ALL_TAC) >>
+        last_x_assum (strip_assume_tac o
+                      REWRITE_RULE [ffi_eq_def,
+                                    BISIM_REL_def,
+                                    BISIM_def]) >>
+        fs[] >>
+        rename1 ‘BR _ _’ >>
+        ‘∃c3 q3 N3.
+          strans conf (cB,q1B,N1B) (ARecv sp d) (c3,q3,N3) ∧
+          BR (cA,q2A,N2A) (c3,q3,N3)’
+          by (fs[pairTheory.FORALL_PROD,
+                 pairTheory.EXISTS_PROD] >>
+              metis_tac[]) >>
+        MAP_EVERY qexists_tac [‘q3’,‘N3’] >>
+        ‘c3 = cB’
+          suffices_by (rw[ffi_eq_def,BISIM_REL_def,
+                          BISIM_def] >>
+                       metis_tac[]) >>
+        metis_tac[strans_pres_pnum,pairTheory.FST]) >>
+  fs[strans_receive_equiv] >>
+  rename[‘RTC (active_trans conf cB) (q1B,N1B) (qIBa,NIB)’,
+         ‘output_trans conf cB (qIBa,NIB) (rp,d) (qIBb,NIB)’,
+         ‘RTC (internal_trans conf cB) (qIBb,NIB) (q2Bb,N2Bb)’] >>
+  ‘ffi_eq conf (cB,qIBb,NIB) (cA,q2A,N2A)’
+    by (‘ffi_eq conf (cB,qIBb,NIB) (cB,q2Bb,N2Bb)’
+          suffices_by metis_tac[ffi_eq_equivRel,equivalence_def,
+                                symmetric_def,transitive_def] >>
+        metis_tac[active_trans_pres_wf,
+                  output_trans_pres_wf,
+                  internal_trans_equiv_irrel]) >>
+  ‘ffi_eq conf (cB,q2B,N2B) (cB,qIBb,NIB)’
+    suffices_by metis_tac[ffi_eq_equivRel,equivalence_def,
+                                symmetric_def,transitive_def] >>
+  drule_all_then strip_assume_tac active_rec_comm >>
+  rename [‘output_trans conf cB (qIBa,NIB) (rp,d) NS’,
+          ‘output_trans conf cB (qIBa,NIB) (rp,d) (qOS,NOS)’] >>
+  PairCases_on ‘NS’ >>
+  ‘qsame NS0 qOS ∧ NS1 = NOS’
+    suffices_by (rw[] >>
+                 ‘ffi_eq conf (cB,q2B,N2B) (cB,NS0,NOS)’
+                  suffices_by metis_tac[qsame_irrel_ffi_eq,
+                                        ffi_eq_equivRel,
+                                        equivalence_def,
+                                        transitive_def] >>
+                 metis_tac[output_trans_pres_wf,
+                           active_trans_equiv_irrel]) >>
+  fs[qsame_def,output_trans_def] >>
+  qpat_x_assum ‘NS0 = NS0 |+ _’ mp_tac >>
+  qpat_x_assum ‘qOS = qOS |+ _’ mp_tac >>
+  qpat_x_assum ‘NS0 |+ _ = qOS |+ _’ mp_tac >>
+  rpt (pop_assum (K ALL_TAC)) >>
+  fs[qlk_def,fget_def] >>
+  rw[] >>
+  reverse (Cases_on ‘sp = rp’)
+  >- metis_tac[finite_mapTheory.FLOOKUP_UPDATE] >>
+  Cases_on ‘FLOOKUP NS0 rp’ >>
+  Cases_on ‘FLOOKUP qOS rp’ >>
+  fs[finite_mapTheory.FLOOKUP_EXT,
+     FUN_EQ_THM] >>
+  last_x_assum (qspec_then ‘rp’ assume_tac) >>
+  fs[finite_mapTheory.FLOOKUP_UPDATE]
+QED
+
+(* EQUIVALENCE PRESERVATION *)
+Theorem ffi_eq_pres:
+  ∀conf SA1 SA2 L SB1 SB2.
+    ffi_wf SA1 ∧
+    ffi_wf SA2 ∧
+    ffi_eq conf SA1 SA2   ∧
+    strans conf SA1 L SB1 ∧
+    strans conf SA2 L SB2   ⇒
+    ffi_eq conf SB1 SB2
+Proof
+  rw[] >>
+  MAP_EVERY PairCases_on [‘SA1’,‘SA2’,‘SB1’,‘SB2’] >>
+  ‘SB10 = SA10 ∧ SB20 = SA20’
+    by metis_tac[pairTheory.FST,strans_pres_pnum] >>
+  Cases_on ‘L’ >>
+  fs[strans_send_equiv,strans_receive_equiv,pairTheory.FST] >>
+  metis_tac[active_trans_equiv_pres,
+            active_trans_pres_wf,
+            send_trans_equiv_pres,
+            input_trans_pres_wf,
+            receive_trans_equiv_pres,
+            output_trans_pres_wf,
+            internal_trans_equiv_pres,
+            internal_trans_pres_wf]
+QED
+
+(* RELATIONSHIP TO COMMUNICATION PROPS *)
+(* Equivalence means same sending destinations *)
+Theorem ffi_eq_sendval:
+  ∀conf x y. ffi_eq conf x y ⇒
+    (∀rp. valid_send_dest rp x ⇔ valid_send_dest rp y)
+Proof
+  rw[EQ_IMP_THM] >>
+  metis_tac[strans_send_cond,strans_dest_check,ffi_eq_def,
+            BISIM_REL_def,BISIM_def]
+QED
+
+(* Equivalence means same receiving capacity *)
+Theorem functional_ARecv:
+  ∀conf x x2a x2b rp msga msgb.
+    ffi_wf x ∧
+    strans conf x (ARecv rp msga) x2a ∧
+    strans conf x (ARecv rp msgb) x2b ⇒
+    msga = msgb
+Proof
+  rw[] >> MAP_EVERY PairCases_on [‘x’,‘x2a’,‘x2b’] >>
+  ‘x2a0 = x0’
+    by metis_tac [strans_pres_pnum,pairTheory.FST] >>
+  ‘x2b0 = x0’
+    by metis_tac [strans_pres_pnum,pairTheory.FST] >>
+  rw[] >>
+  fs[strans_receive_equiv] >>
+  rename [‘msga = msgb’,
+          ‘RTC (active_trans conf x0) (x1,x2) (qi1a,nia)’,
+          ‘output_trans conf x0 (qi1a,nia) (rp,msga) (qi2a,nia)’,
+          ‘RTC (active_trans conf x0) (x1,x2) (qi1b,nib)’,
+          ‘output_trans conf x0 (qi1b,nib) (rp,msgb) (qi2b,nib)’] >>
+  ‘∃qC nC. RTC (active_trans conf x0) (qi1a,nia) (qC,nC) ∧
+           RTC (active_trans conf x0) (qi1b,nib) (qC,nC)’
+    by (rw[GSYM pairTheory.EXISTS_PROD] >>
+        irule active_active_comm >>
+        metis_tac[]) >>
+  ‘∃qFA nFA. output_trans conf x0 (qC,nC) (rp,msga) (qFA,nFA) ∧
+             RTC (active_trans conf x0) (qi2a,nia) (qFA,nFA)’
+    by (rw[GSYM pairTheory.EXISTS_PROD] >>
+        irule active_rec_comm >>
+        metis_tac[active_trans_pres_wf]) >>
+  ‘∃qFB nFB. output_trans conf x0 (qC,nC) (rp,msgb) (qFB,nFB) ∧
+             RTC (active_trans conf x0) (qi2b,nib) (qFB,nFB)’
+    by (rw[GSYM pairTheory.EXISTS_PROD] >>
+        irule active_rec_comm >>
+        metis_tac[active_trans_pres_wf]) >>
+  rpt (qpat_x_assum ‘output_trans _ _ (qC,nC) _ _’ mp_tac) >>
+  rpt (pop_assum (K ALL_TAC)) >>
+  rw[output_trans_def] >>
+  pop_assum (K ALL_TAC) >>
+  last_x_assum (K ALL_TAC) >>
+  fs[finite_mapTheory.FLOOKUP_EXT,FUN_EQ_THM] >>
+  pop_assum (qspec_then ‘rp’ assume_tac) >>
+  fs[finite_mapTheory.FLOOKUP_UPDATE]
+QED
+
+Theorem ffi_eq_ARecv:
+  ∀conf x y x2 y2 rp msga msgb.
+    ffi_wf x ∧
+    ffi_eq conf x y ∧
+    strans conf x (ARecv rp msga) x2 ∧
+    strans conf y (ARecv rp msgb) y2 ⇒
+    msga = msgb
+Proof
+  CCONTR_TAC >> fs[] >>
+  ‘∃x2b. strans conf x (ARecv rp msgb) x2b’
+    suffices_by metis_tac[functional_ARecv] >>
+  metis_tac[ffi_eq_def,BISIM_REL_def,BISIM_def]
+QED
+
+Theorem some_satisfies_cond:
+  ∀P. (some x. P x) = SOME z ⇒ P z
+Proof
+  rw[some_def] >> SELECT_ELIM_TAC >>
+  metis_tac[]
+QED
+
+Theorem ffi_eq_receives:
+  ∀conf x y.
+    ffi_wf x.ffi_state ∧
+    ffi_wf y.ffi_state ∧
+    x.oracle = comms_ffi_oracle conf ∧
+    y.oracle = comms_ffi_oracle conf ∧
+    ffi_eq conf x.ffi_state y.ffi_state ⇒
+    ffi_receives conf x = ffi_receives conf y
+Proof
+  simp[FUN_EQ_THM,PULL_FORALL] >>
+  rpt gen_tac >>
+  rename1 ‘ffi_receives conf x src msg = ffi_receives conf y src msg’ >>
+  MAP_EVERY qid_spec_tac [‘y’,‘x’] >>
+  completeInduct_on ‘LENGTH msg’ >>
+  rw[Once ffi_receives_def] >>
+  qmatch_goalsub_abbrev_tac ‘LP ⇔ _’ >>
+  rw[Once ffi_receives_def] >>
+  qunabbrev_tac ‘LP’ >>
+  qmatch_goalsub_abbrev_tac ‘PA ∧ PB ∧ PCA ⇔ PA ∧ PB ∧ PCB’ >>
+  ‘PCA ⇔ PCB’
+    suffices_by rw[] >>
+  MAP_EVERY qunabbrev_tac [‘PA’,‘PB’,‘PCA’,‘PCB’] >>
+  rw[EQ_IMP_THM] >>
+  first_x_assum (drule_all_then strip_assume_tac) >>
+  rw[]
+  >- (rfs[call_FFI_def,valid_receive_call_format_def,
+         comms_ffi_oracle_def,ffi_receive_def] >>
+      DEEP_INTRO_TAC some_intro >> rw[] >>
+      Cases_on ‘some (m,ns). (strans conf x.ffi_state (ARecv param m) ns)’ >>
+      fs[] >>
+      rename1 ‘(some (m,ns). strans conf x.ffi_state (ARecv param m) ns) = SOME nsb’ >>
+      ‘(λ(m,ns). strans conf x.ffi_state (ARecv param m) ns) nsb’
+            by metis_tac[some_satisfies_cond] >>
+      PairCases_on ‘nsb’ >> fs[]
+      >- (rename1 ‘(λ(m,ns). strans conf y.ffi_state (ARecv param m) ns) ns’ >>
+          PairCases_on ‘ns’ >>
+          Cases_on ‘LENGTH ns0 = SUC conf.payload_size’ >> fs[] >>
+          ‘nsb0 = ns0’
+            by metis_tac[ffi_eq_ARecv] >>
+          fs[])
+      >- (rw[pairTheory.EXISTS_PROD] >>
+          qexists_tac ‘nsb0’ >>
+          rw[GSYM pairTheory.EXISTS_PROD] >>
+          qabbrev_tac ‘L = ARecv param nsb0’ >>
+          qabbrev_tac ‘x2 = (nsb1,nsb2,nsb3)’ >>
+          metis_tac[ffi_eq_def,BISIM_REL_def,BISIM_def]))
+  >- (rfs[call_FFI_def,valid_receive_call_format_def,
+         comms_ffi_oracle_def,ffi_receive_def] >>
+      DEEP_INTRO_TAC some_intro >> rw[] >>
+      Cases_on ‘some (m,ns). (strans conf x.ffi_state (ARecv param m) ns)’ >>
+      fs[] >>
+      rename1 ‘(some (m,ns). strans conf x.ffi_state (ARecv param m) ns) = SOME nsb’ >>
+      ‘(λ(m,ns). strans conf x.ffi_state (ARecv param m) ns) nsb’
+            by metis_tac[some_satisfies_cond] >>
+      PairCases_on ‘nsb’ >> fs[]
+      >- (rename1 ‘(λ(m,ns). strans conf y.ffi_state (ARecv param m) ns) ns’ >>
+          PairCases_on ‘ns’ >> fs[] >>
+          ‘nsb0 = ns0’
+            by metis_tac[ffi_eq_ARecv] >>
+          fs[] >> Cases_on ‘LENGTH ns0 = SUC conf.payload_size’ >> fs[] >>
+          DISJ2_TAC >>
+          last_x_assum (qspec_then ‘LENGTH (DROP conf.payload_size msg)’ assume_tac) >>
+          rfs[] >> first_x_assum (qspec_then ‘DROP conf.payload_size msg’ assume_tac) >>
+          rfs[] >> qmatch_goalsub_abbrev_tac ‘ffi_receives _ nstY _ _’ >>
+          first_x_assum (qspecl_then [‘nst’,‘nstY’] assume_tac) >>
+          rfs[] >> pop_assum irule >>
+          qunabbrev_tac ‘nstY’ >>
+          qpat_x_assum ‘_ = nst’ (SUBST1_TAC o GSYM) >>
+          rw[] >> metis_tac[strans_pres_wf,ffi_eq_pres])
+      >- (rw[pairTheory.EXISTS_PROD] >>
+          qexists_tac ‘nsb0’ >>
+          rw[GSYM pairTheory.EXISTS_PROD] >>
+          qabbrev_tac ‘L = ARecv param nsb0’ >>
+          qabbrev_tac ‘x2 = (nsb1,nsb2,nsb3)’ >>
+          metis_tac[ffi_eq_def,BISIM_REL_def,BISIM_def]))
+  >- (rfs[call_FFI_def,valid_receive_call_format_def,
+         comms_ffi_oracle_def,ffi_receive_def] >>
+      DEEP_INTRO_TAC some_intro >> rw[] >>
+      Cases_on ‘some (m,ns). (strans conf y.ffi_state (ARecv param m) ns)’ >>
+      fs[] >>
+      rename1 ‘(some (m,ns). strans conf y.ffi_state (ARecv param m) ns) = SOME nsb’ >>
+      ‘(λ(m,ns). strans conf y.ffi_state (ARecv param m) ns) nsb’
+            by metis_tac[some_satisfies_cond] >>
+      PairCases_on ‘nsb’ >> fs[]
+      >- (rename1 ‘(λ(m,ns). strans conf x.ffi_state (ARecv param m) ns) ns’ >>
+          PairCases_on ‘ns’ >>
+          Cases_on ‘LENGTH ns0 = SUC conf.payload_size’ >> fs[] >>
+          ‘nsb0 = ns0’
+            by metis_tac[ffi_eq_ARecv] >>
+          fs[])
+      >- (rw[pairTheory.EXISTS_PROD] >>
+          qexists_tac ‘nsb0’ >>
+          rw[GSYM pairTheory.EXISTS_PROD] >>
+          qabbrev_tac ‘L = ARecv param nsb0’ >>
+          qabbrev_tac ‘y2 = (nsb1,nsb2,nsb3)’ >>
+          metis_tac[ffi_eq_def,BISIM_REL_def,BISIM_def]))
+  >- (rfs[call_FFI_def,valid_receive_call_format_def,
+         comms_ffi_oracle_def,ffi_receive_def] >>
+      DEEP_INTRO_TAC some_intro >> rw[] >>
+      Cases_on ‘some (m,ns). (strans conf y.ffi_state (ARecv param m) ns)’ >>
+      fs[] >>
+      rename1 ‘(some (m,ns). strans conf y.ffi_state (ARecv param m) ns) = SOME nsb’ >>
+      ‘(λ(m,ns). strans conf y.ffi_state (ARecv param m) ns) nsb’
+            by metis_tac[some_satisfies_cond] >>
+      PairCases_on ‘nsb’ >> fs[]
+      >- (rename1 ‘(λ(m,ns). strans conf x.ffi_state (ARecv param m) ns) ns’ >>
+          PairCases_on ‘ns’ >> fs[] >>
+          ‘nsb0 = ns0’
+            by metis_tac[ffi_eq_ARecv] >>
+          fs[] >> Cases_on ‘LENGTH ns0 = SUC conf.payload_size’ >> fs[] >>
+          DISJ2_TAC >>
+          last_x_assum (qspec_then ‘LENGTH (DROP conf.payload_size msg)’ assume_tac) >>
+          rfs[] >> first_x_assum (qspec_then ‘DROP conf.payload_size msg’ assume_tac) >>
+          rfs[] >> qmatch_goalsub_abbrev_tac ‘ffi_receives _ nstX _ _’ >>
+          first_x_assum (qspecl_then [‘nst’,‘nstX’] assume_tac) >>
+          rfs[] >> pop_assum irule >>
+          qunabbrev_tac ‘nstX’ >>
+          qpat_x_assum ‘_ = nst’ (SUBST1_TAC o GSYM) >>
+          rw[] >>
+          metis_tac[strans_pres_wf,ffi_eq_pres,ffi_eq_equivRel,
+                    equivalence_def,symmetric_def])
+      >- (rw[pairTheory.EXISTS_PROD] >>
+          qexists_tac ‘nsb0’ >>
+          rw[GSYM pairTheory.EXISTS_PROD] >>
+          qabbrev_tac ‘L = ARecv param nsb0’ >>
+          qabbrev_tac ‘y2 = (nsb1,nsb2,nsb3)’ >>
+          metis_tac[ffi_eq_def,BISIM_REL_def,BISIM_def]))
+QED
+
+val _ = export_theory ();
