projection/proofs/to_cake/ffi/comms_ffi_modelScript.sml
@@ -1,0 +1,85 @@
+open HolKernel boolLib Parse bossLib;
+open ffiTheory;
+open payloadSemTheory;
+
+val _ = new_theory "comms_ffi_model";
+
+(* FFI MODEL *)
+(* Static Model
+    Basic model off FFI or World state at any
+    given point in time *)
+(* -- Backend Queues *)
+Type queues = “: proc |-> datum list”;
+(* -- Total FFI State model *)
+Type total_state = “: proc # queues # network”;
+
+(* Transition System
+    Describes possible transitions of the
+    static FFI type based on interaction*)
+(* -- FFI interaction actions *)
+Datatype:
+ action = ASend proc datum
+          | ARecv proc datum
+End
+(* -- Transition system on FFI states *)
+Inductive strans:
+  (* ARecv *)
+  (∀conf c q ms mc tl N.
+    qlk q ms = mc::tl
+    ⇒ strans conf (c,q,N) (ARecv ms mc) (c,q |+ (ms,tl), N)) ∧
+
+  (* LTauL *)
+  (∀conf c q q' N N' N'' α.
+     trans conf N LTau N' ∧
+     strans conf (c,q,N') α (c,q',N'')
+     ⇒  strans conf (c,q,N) α (c,q',N'')) ∧
+
+  (* LTauR *)
+  (∀conf c q q' N N' N'' α.
+     strans conf (c,q,N) α (c,q',N') ∧
+     trans conf N' LTau N''
+     ⇒  strans conf (c,q,N) α (c,q',N'')) ∧
+
+  (* LSend *)
+  (∀conf c q q' N N' N'' sp d α.
+     trans conf N (LSend sp d c) N' ∧
+     strans conf (c,qpush q sp d,N') α (c,q',N'')
+     ⇒  strans conf (c,q,N) α (c,q',N'')) ∧
+
+  (* ASend *)
+  (∀conf c q N N' rp d.
+     trans conf N (LReceive c d rp) N'
+     ⇒  strans conf (c,q,N) (ASend rp d) (c,q,N'))
+End
+
+(* Dynamic Model
+     Model of response to FFI calls based on transition system *)
+(* -- send call model *)
+Definition ffi_send_def:
+  ffi_send conf os dest data =
+  if (LENGTH data ≠ SUC conf.payload_size) then
+    Oracle_final FFI_failed
+  else
+    case some ns. strans conf os (ASend dest data) ns of
+      SOME ns =>  Oracle_return ns data
+    | NONE    =>  Oracle_final FFI_diverged
+End
+(* -- receive call model *)
+Definition ffi_receive_def:
+  ffi_receive conf os src _ =
+    case some (m,ns). strans conf os (ARecv src m) ns of
+      SOME (m,ns) =>  Oracle_return ns m
+    | NONE        =>  Oracle_final FFI_diverged
+End
+(* -- total oracle *)
+Definition comms_ffi_oracle_def:
+  comms_ffi_oracle conf name =
+    if name = "send" then
+        ffi_send conf
+    else if name = "receive" then
+        ffi_receive conf
+    else
+        (λ _ _ _. Oracle_final FFI_failed)
+End
+
+val _ = export_theory ();
