projection/proofs/to_cake/theory_tools/ckExp_EquivScript.sml
@@ -1,0 +1,325 @@
+open HolKernel boolLib Parse bossLib;
+open semanticPrimitivesTheory
+     evaluateTheory
+     terminationTheory
+     evaluatePropsTheory
+     ml_translatorTheory;
+open evaluate_toolsTheory
+     evaluate_rwLib;
+
+val _ = new_theory "ckExp_Equiv";
+
+val WORD8 = “WORD:word8 -> v -> bool”;
+
+(* UNIQUE CORRECT TRANSLATION FRAMEWORK *)
+(* Basic Injective HOL, CakeML mapping constraint
+   (Unique Correct Translation *)
+Definition UNCT_def:
+  UNCT (tf:α -> v -> bool) = ∀(a:α) (v1 v2:v). tf a v1 ∧ tf a v2 ⇒ v1 = v2
+End
+
+(* Preexistent UNCT maps *)
+Theorem INT_UNCT:
+  UNCT INT
+Proof
+  rw[UNCT_def,INT_def] 
+QED
+
+Theorem NUM_UNCT:
+  UNCT NUM
+Proof
+  rw[UNCT_def,NUM_def,INT_def] 
+QED
+
+Theorem BOOL_UNCT:
+  UNCT BOOL
+Proof
+  rw[UNCT_def,BOOL_def]
+QED
+
+Theorem WORD_UNCT:
+  UNCT WORD
+Proof
+  rw[UNCT_def,WORD_def]
+QED
+
+Theorem CHAR_UNCT:
+  UNCT CHAR
+Proof
+  rw[UNCT_def,CHAR_def]
+QED
+
+Theorem STRING_TYPE_UNCT:
+  UNCT STRING_TYPE
+Proof
+  rw[UNCT_def] >>
+  Cases_on ‘a’ >>
+  fs[STRING_TYPE_def]
+QED
+
+(* -- List version of UNCT type is UNCT *)
+Theorem LIST_TYPE_UNCT:
+  ∀tf.
+    UNCT tf ⇒ UNCT (LIST_TYPE tf)
+Proof
+  simp[UNCT_def] >>
+  strip_tac >>
+  strip_tac >>
+  Induct_on ‘a’
+  >- rw[LIST_TYPE_def]
+  >- (rpt strip_tac >>
+      fs[LIST_TYPE_def] >>
+      metis_tac[])
+QED
+
+
+(* BASIC CAKEML EXP TO HOL EQUIVALENCE FRAMEWORK *)
+(* Basic Definition of CakeML Expression/HOL Term equivalence *)
+Definition ck_equiv_hol_def:
+  ck_equiv_hol cEnv hT cExp hVal =
+    ∀arefs.
+      ∃bc1 bc2 drefs cVal.
+        hT hVal cVal ∧
+        evaluate (empty_state with <|clock := bc1; refs := arefs|>) cEnv [cExp] = 
+          (empty_state with <|clock := bc2; refs := arefs ++ drefs|>,
+          Rval [cVal])
+End
+
+(* Methods of applying equivalence *)
+(* -- Application of equivalence to produce
+      equivalent result in arbtirary state *)
+Theorem ck_equiv_hol_apply:
+  ∀ cEnv hT cExp hV.
+    ck_equiv_hol cEnv hT cExp hV ⇒
+      ∀cSt.
+        ∃bc1 bc2 drefs cV.
+          hT hV cV ∧
+          ∀dc.
+            evaluate (cSt with clock := bc1 + dc) cEnv [cExp]
+            = (cSt with <|clock := dc + bc2;
+                          refs := cSt.refs ++ drefs|>,
+                      Rval [cV])
+Proof
+  rpt strip_tac >>
+  fs[ck_equiv_hol_def] >>
+  first_x_assum (qspec_then ‘cSt.refs’ strip_assume_tac) >>
+  MAP_EVERY qexists_tac [‘bc1’,‘bc2’,‘drefs’,‘cVal’] >>
+  simp[evaluate_generalise]
+QED
+
+(* -- Identical to original but quantifiers moved.
+      This is useful because if polymorphic theorems
+      (cSt can have any FFI model type) are introduced
+      in a HOL proof without being fully intialised they
+      are given arbitrary fixed types. So state is at
+      top to be specialised at the beginning. *)
+Theorem ck_equiv_hol_apply_alt:
+  ∀ cEnv hT cExp hV cSt.
+    ck_equiv_hol cEnv hT cExp hV ⇒
+      ∃bc1 bc2 drefs cV.
+        hT hV cV ∧
+        ∀dc.
+          evaluate (cSt with clock := bc1 + dc) cEnv [cExp]
+          = (cSt with <|clock := dc + bc2;
+                        refs := cSt.refs ++ drefs|>,
+                    Rval [cV])
+Proof
+  rw[] >>
+  drule_then (qspec_then ‘cSt’ strip_assume_tac) ck_equiv_hol_apply >>
+  MAP_EVERY qexists_tac [‘bc1’,‘bc2’,‘drefs’,‘cV’] >>
+  simp[]
+QED
+
+(* -- Swap Expression in Function argument with equivalent literal *)
+Theorem ck_equiv_hol_apply_lit_App:
+  ∀fexp aexp hT hA cEnv cL.
+    UNCT hT                      ∧
+    hT hA (Litv cL)              ∧
+    ck_equiv_hol cEnv hT aexp hA
+     ⇒
+    ∀cSt.
+        ∃mc1 mc2 drefs.
+          ∀dc.
+            evaluate (cSt with clock := mc1 + dc) cEnv [App Opapp [fexp;aexp]]
+            = evaluate (cSt with <|clock := mc2 + dc; refs := cSt.refs ++ drefs|>) cEnv
+              [App Opapp [fexp; Lit cL]]
+Proof
+  rpt strip_tac >>
+  rw[evaluate_def] >>
+  qpat_x_assum ‘ck_equiv_hol cEnv hT aexp hA’ assume_tac >>
+  drule_then (qspec_then ‘cSt’ strip_assume_tac) ck_equiv_hol_apply >>
+  rename1 ‘∀dc.
+            evaluate (cSt with clock := bc1_a + dc) cEnv [aexp] =
+            (cSt with <|clock := dc + bc2_a; refs := cSt.refs ++ drefs_a|>,
+             Rval [cV])’ >>
+  Q.REFINE_EXISTS_TAC ‘bc1_a + mc1’ >>
+  simp[] >>
+  MAP_EVERY qexists_tac [‘0’,‘bc2_a’,‘drefs_a’] >>
+  ‘Litv cL = cV’
+    suffices_by simp[] >>
+  metis_tac[UNCT_def]
+QED
+
+(* Methods of constructing equivalence *)
+(* -- Literals *)
+Theorem ck_equiv_hol_Lit:
+  ∀hT cL cEnv hL.
+    hT hL (Litv cL) ⇒
+    ck_equiv_hol cEnv hT (Lit cL) hL
+Proof
+  rpt strip_tac >>
+  rw[ck_equiv_hol_def,evaluate_def] >>
+  MAP_EVERY qexists_tac [‘0’,‘0’,‘[]’] >>
+  rw[]
+QED
+
+(* -- Variables *)
+Theorem ck_equiv_hol_Var:
+  ∀cEnv vid hT hV.
+    (∃cV. nsLookup cEnv.v vid = SOME cV ∧
+          hT hV cV) ⇒
+    ck_equiv_hol cEnv hT (Var vid) hV
+Proof
+  rpt strip_tac >>
+  rw[ck_equiv_hol_def,evaluate_def] >>
+  MAP_EVERY qexists_tac [‘0’,‘0’,‘[]’] >>
+  rw[]
+QED
+
+(* -- Function Application *)
+Theorem ck_equiv_hol_App:
+  ∀fexp hf aexp ha tA tB cEnv.
+    ck_equiv_hol cEnv tA aexp ha          ∧
+    ck_equiv_hol cEnv (tA --> tB) fexp hf ⇒
+    ck_equiv_hol cEnv tB (App Opapp [fexp;aexp]) (hf ha)
+Proof
+  rpt strip_tac >>
+  rw[ck_equiv_hol_def] >>
+  fs[ck_equiv_hol_def] >>
+  rw [evaluate_def] >>
+  last_x_assum (qspec_then ‘arefs’ strip_assume_tac) >>
+  rename1 ‘evaluate (empty_state with <|clock := bc1_a; refs := arefs|>) cEnv
+                   [aexp] = (empty_state with <|clock := bc2_a;
+                                                refs := arefs ++ drefs_a|>,
+                             Rval [cVal_a])’ >>
+  Q.REFINE_EXISTS_TAC ‘bc1_a + bc1’ >>
+  ‘∀bc1. evaluate (empty_state with <|clock := bc1_a + bc1; refs := arefs|>) cEnv
+                   [aexp] = (empty_state with <|clock := bc2_a + bc1;
+                                                refs := arefs ++ drefs_a|>,
+                             Rval [cVal_a])’
+    by (rpt strip_tac >>
+        qspecl_then [‘empty_state with <|clock := bc1_a;
+                                         refs := arefs|>’,
+                     ‘cEnv’, ‘[aexp]’,
+                     ‘empty_state with <|clock := bc2_a;
+                                         refs := arefs ++ drefs_a|>’,
+                     ‘Rval [cVal_a]’, ‘bc1’]
+                assume_tac evaluate_add_to_clock >>
+        rfs[]) >>
+  rfs[] >>
+  ntac 2 (first_x_assum (K ALL_TAC)) >>
+  last_x_assum (qspec_then ‘arefs ++ drefs_a’ strip_assume_tac) >>
+  rename1 ‘evaluate (empty_state with <|clock := bc1_f;
+                                        refs := arefs ++ drefs_a|>)
+                    cEnv [fexp] = (empty_state with <|clock := bc2_f;
+                                                      refs  := arefs
+                                                               ++ drefs_a
+                                                               ++ drefs_f|>,
+                                   Rval [cVal_f])’ >>
+  Q.REFINE_EXISTS_TAC ‘bc1_f + bc1’ >>
+  ‘∀bc1. evaluate (empty_state with <|clock := bc1_f + bc1 + bc2_a;
+                                refs := arefs ++ drefs_a|>)
+            cEnv
+            [fexp] = (empty_state with <|clock := bc2_f + bc1 + bc2_a;
+                                         refs  := arefs ++ drefs_a ++ drefs_f|>,
+                      Rval [cVal_f])’
+    by (rpt strip_tac >>
+        qspecl_then [‘empty_state with <|clock := bc1_f;
+                                         refs := arefs ++ drefs_a|>’,
+                     ‘cEnv’, ‘[fexp]’,
+                     ‘empty_state with <|clock := bc2_f;
+                                         refs := arefs ++ drefs_a ++ drefs_f|>’,
+                     ‘Rval [cVal_f]’, ‘bc1 + bc2_a’]
+                assume_tac evaluate_add_to_clock >>
+        rfs[]) >>
+  rfs[] >>
+  ntac 2 (first_x_assum (K ALL_TAC)) >>
+  qspecl_then [‘cVal_f’,‘hf’,‘ha’,‘cVal_a’,‘tA’,‘tB’,
+               ‘empty_state with <|refs := arefs ++ drefs_a ++ drefs_f|>’]
+  strip_assume_tac do_opapp_translate >>
+  rfs[] >>
+  rename1 ‘∀dc.
+            evaluate
+              (empty_state with
+               <|clock := bc1 + dc; refs := arefs ++ drefs_a ++ drefs_f|>)
+              cfa_env [cfa_exp] =
+            (empty_state with
+             <|clock := bc2 + dc;
+               refs := arefs ++ drefs_a ++ drefs_f ++ drefs|>,Rval [crv])’ >>
+  MAP_EVERY qexists_tac [‘SUC bc1’,‘bc2+(bc2_a+bc2_f)’,‘drefs_a ++ drefs_f ++ drefs’,‘crv’] >>
+  rw[arithmeticTheory.ADD1,dec_clock_def]
+QED
+
+(* -- Equality of byte arrays/lists *)
+Theorem ck_equiv_hol_apply_list_word8_equality:
+  ∀cEnv aexp hA bexp hB.
+    ck_equiv_hol cEnv (LIST_TYPE ^WORD8) aexp hA ∧
+    ck_equiv_hol cEnv (LIST_TYPE ^WORD8) bexp hB   ⇒
+    ck_equiv_hol cEnv BOOL (App Equality [aexp;bexp]) (hA = hB)
+Proof
+  rpt strip_tac >>
+  rw [ck_equiv_hol_def] >>
+  CONV_TAC (RESORT_EXISTS_CONV rev) >>
+  MAP_EVERY qexists_tac [‘Boolv (hA = hB)’] >>
+  simp trans_sl >>
+  CONV_TAC (RESORT_EXISTS_CONV rev) >>
+  qmatch_goalsub_abbrev_tac ‘evaluate (cSt with clock := _) _ _’ >>
+  qspecl_then [‘cEnv’,‘LIST_TYPE ^WORD8’,‘bexp’,‘hB’,‘cSt’]
+              strip_assume_tac ck_equiv_hol_apply_alt >>
+  rfs[] >>
+  Q.REFINE_EXISTS_TAC ‘bc1 + r1’ >>
+  rw eval_sl >>
+  qpat_x_assum ‘∀dc. P dc’ (K ALL_TAC) >>
+  qunabbrev_tac ‘cSt’ >>
+  simp [] >>
+  qmatch_goalsub_abbrev_tac ‘evaluate (cSt with clock := _) _ _’ >>
+  qspecl_then [‘cEnv’,‘LIST_TYPE ^WORD8’,‘aexp’,‘hA’,‘cSt’]
+              strip_assume_tac ck_equiv_hol_apply_alt >>
+  rfs[] >>
+  Q.REFINE_EXISTS_TAC ‘bc1 + r1’ >>
+  simp[] >>
+  qpat_x_assum ‘∀dc. P dc’ (K ALL_TAC)
+  >- (‘cV' = cV’
+        by metis_tac[UNCT_def,LIST_TYPE_UNCT,WORD_UNCT] >>
+      fs[] >>
+      first_x_assum (K ALL_TAC) >>
+      ‘∀hL cL. LIST_TYPE ^WORD8 hL cL ⇒ (do_eq cL cL = Eq_val T)’
+        suffices_by (qunabbrev_tac ‘cSt’ >> rw[] >> ‘do_eq cV cV = Eq_val T’ by metis_tac[] >>
+                     simp[] >> MAP_EVERY qexists_tac [‘0’,‘bc2 + bc2'’,‘drefs ++ drefs'’] >>
+                     simp[state_component_equality]) >>
+      Induct_on ‘hL’
+      >- (rw trans_sl >> EVAL_TAC)
+      >- (Cases_on ‘cL’ >> rw [do_eq_def,LIST_TYPE_def] >>
+          rw [do_eq_def] >> Cases_on ‘v2_1’ >> fs[do_eq_def,WORD_def]))
+  >- (‘∀hAt cAt hBt cBt.
+        LIST_TYPE ^WORD8 hAt cAt ∧
+        LIST_TYPE ^WORD8 hBt cBt ∧
+        hAt ≠ hBt ⇒
+        (do_eq cAt cBt = Eq_val F)’
+        suffices_by (qunabbrev_tac ‘cSt’ >> rw[] >> ‘do_eq cV' cV = Eq_val F’ by metis_tac[] >>
+                     simp[] >> MAP_EVERY qexists_tac [‘0’,‘bc2 + bc2'’,‘drefs ++ drefs'’] >>
+                     simp[state_component_equality]) >>
+      Induct_on ‘hAt’
+      >- (rw[LIST_TYPE_def] >> Cases_on ‘hBt’ >> fs [] >>
+          fs[LIST_TYPE_def] >> rw[do_eq_def] >>
+          fs[ctor_same_type_def,same_type_def])
+      >- (rw[LIST_TYPE_def] >> Cases_on ‘hBt’ >> fs[LIST_TYPE_def] >>
+          rw[do_eq_def] >> fs[ctor_same_type_def,same_type_def] >>
+          Cases_on ‘v2_1’ >> Cases_on ‘v2_1'’ >> fs trans_sl >>
+          rw[do_eq_def] >> fs[lit_same_type_def,same_type_def] >>
+          ‘do_eq v2_2 v2_2' = Eq_val F’
+            by metis_tac[] >>
+          Cases_on ‘h = h'’ >> simp[]))
+QED
+
+val _ = export_theory()
